@prefix schema: <http://schema.org/> .
@prefix adms: <http://www.w3.org/ns/adms#> .
@prefix owl: <http://www.w3.org/2002/07/owl#> .
@prefix org: <http://www.w3.org/ns/org#> .
@prefix xls2rdf: <https://xls2rdf.sparna.fr/vocabulary#> .
@prefix xsd: <http://www.w3.org/2001/XMLSchema#> .
@prefix skosthes: <http://purl.org/iso25964/skos-thes#> .
@prefix rdfs: <http://www.w3.org/2000/01/rdf-schema#> .
@prefix qb: <http://purl.org/linked-data/cube#> .
@prefix cv: <http://data.europa.eu/m8g/> .
@prefix dct: <http://purl.org/dc/terms/> .
@prefix rdf: <http://www.w3.org/1999/02/22-rdf-syntax-ns#> .
@prefix doap: <http://usefulinc.com/ns/doap#> .
@prefix sh: <http://www.w3.org/ns/shacl#> .
@prefix vann: <http://purl.org/vocab/vann/> .
@prefix dcat: <http://www.w3.org/ns/dcat#> .
@prefix euvoc: <http://publications.europa.eu/ontology/euvoc#> .
@prefix prov: <http://www.w3.org/ns/prov#> .
@prefix foaf: <http://xmlns.com/foaf/0.1/> .
@prefix dc: <http://purl.org/dc/elements/1.1/> .
@prefix skos: <http://www.w3.org/2004/02/skos/core#> .
@prefix skosxl: <http://www.w3.org/2008/05/skos-xl#> .

<http://data.europa.eu/m8g/cpsvap/3.2.0> a owl:Ontology;
  vann:preferredNamespaceURI "http://data.europa.eu/m8g/cpsvap";
  vann:preferredNamespacePrefix "cpsvap";
  dct:title "CPSV-AP";
  dct:description "The Core Public Service Vocabulary Application Profile (CPSV-AP) is a reusable and extensible data specification used for harmonising the way public services are described in a machine-readable format. CPSV-AP captures fundamental characteristics of a public service, such as the name, description, competent public organisation, output, etc. Public administrations and service providers can therefore use this approach to describe their services and guarantee a level of cross-domain and cross-border interoperability at European, national and local level.";
  owl:versionIRI <http://data.europa.eu/m8g/cpsvap/3.2.0>;
  owl:versionInfo "3.2.0";
  dct:created "2024-01-31"^^xsd:date;
  dct:creator <http://publications.europa.eu/resource/authority/corporate-body/DIGIT>;
  dct:license <https://creativecommons.org/licenses/by/4.0/>;
  rdfs:seeAlso <https://joinup.ec.europa.eu/asset/cpsv-ap/home> .

<http://purl.org/vocab/cpsv#PublicService> a owl:Class;
  rdfs:comment "A Public Service is a mandatory or discretionary set of activities performed, or able to be performed, by or on behalf of a public organisation, publicly funded and arise from public policy."@en;
  rdfs:label "Public Service"@en;
  skos:scopeNote "This class represents the Public Service itself, as it is described in a public service catalogue. Services may be for the benefit of an individual, a business, or other public authority, or groups of any of these. A service exists whether it is used or not, and the term 'benefit' may apply in the sense of enabling the fulfilment of an obligation. As defined in the revised version of the European Interoperability Framework, a European public service comprises any service provided by public administrations in Europe, or by other organisations on their behalf, to businesses, citizens or others public administrations."@en .

dct:audience a owl:ObjectProperty;
  rdfs:comment "The target recipient of the Public Service."@en;
  rdfs:label "addressee"@en;
  skos:scopeNote "Examples are citizens, business, etc."@en .

dct:description a owl:DatatypeProperty;
  rdfs:comment "A free text Description of the Public Service."@en, "A free text Description of the Rule."@en,
    "A free text description of the Channel, for example to describe conditions when to use it."@en,
    "A free text description of the Cost."@en, "A free text description of the Event."@en,
    "A free text Description of the piece of Evidence."@en, "A free text Description of the Output."@en,
    "A textual explanation of the Participation."@en, "A free text description of the Service Concession Contract."@en,
    "A free-text account of the Dataset. This property can be repeated for parallel language versions of the description."@en,
    "A textual representation of the Temporal Entity."@en;
  rdfs:label "description"@en;
  skos:scopeNote "The description is likely to be the text that potential users of the Public Service see in any public service catalogue. Public administrations are encouraged to include a reasonable level of detail in the description, for instance including basic eligibility requirements for the particular Public Service and contact information."@en,
    "The description is likely to be the text that a business or citizen sees for that specific Event when looking for relevant Public Services. Public administrations are therefore encouraged to include a reasonable level of detail in the description."@en .

dct:type a owl:ObjectProperty;
  rdfs:comment "The purpose of a government activity, which the public service is intended for."@en,
    "Type of Rule."@en, "It links an Event to a controlled vocabulary of event types."@en,
    "The type of Channel as defined in a controlled vocabulary."@en, "The type of Evidence as described in a controlled vocabulary."@en,
    "The type of Output as defined in a controlled vocabulary."@en, "Category to which the Requirement belongs."@en;
  rdfs:label "functions of government"@en, "type"@en;
  skos:scopeNote "The possible values for this property are described in the controlled vocabulary <a href=\" https://op.europa.eu/en/web/eu-vocabularies/concept-scheme/-/resource?uri=http://publications.europa.eu/resource/authority/main-activity\">COFOG main activity</a> Authority Table of the Publications Office."@en,
    "For example: a rule for non-disclosure of a dataset, a rule for disclosure of a dataset, etc."@en,
    "The recommended Controlled vocabulary to be used is the <a href=\"https://op.europa.eu/en/web/eu-vocabularies/dataset/-/resource?uri=http://publications.europa.eu/resource/dataset/business-event\">Business Event</a> Vocabulary maintained by the Publications Office of the EU."@en,
    """The recommended controlled vocabularies for this property is the <a href=\"https://op.europa.eu/en/web/eu-vocabularies/concept-scheme/-/resource?uri=http://data.europa.eu/snb/com-channel/25831c2\">Europass Channel Type</a> Authority Table of the Publications Office.

Member States could create subclasses of Channel by adding a e-mail address or an homepage depending on the channel type, in this case VCard could be eventually used."""@en,
    "The recommended Controlled vocabulary to be used is the <a href=\"https://op.europa.eu/en/web/eu-vocabularies/dataset/-/resource?uri=http://publications.europa.eu/resource/dataset/life-event\">Life Events</a> Vocabulary maintained by the Publications Office of the EU."@en,
    "Possible values of Output types are: Declaration, Physical object, Code, Financial obligation, Financial benefit, Recognition, Permit."@en .

dct:identifier a owl:DatatypeProperty;
  rdfs:comment "A formally-issued Identifier for the Public Service."@en, "An Identifier for the Rule."@en,
    "An Identifier for the Channel."@en, "An Identifier for the Cost."@en, "An Identifier for the Event."@en,
    "An Identifier for the piece of Evidence."@en, "Unambiguous reference to the Evidence Type."@en,
    "An Identifier for the Output."@en, "The unambiguous structured reference for the Participation."@en,
    "Unambiguous reference to a Requirement."@en, "An Identifier for the Service Concession Contract."@en,
    "The main identifier for the Dataset, e.g. the URI or other unique identifier in the context of the Catalogue."@en,
    "An Identifier for the Agent."@en;
  rdfs:label "identifier"@en .

dcat:keyword a owl:DatatypeProperty;
  rdfs:comment "A keyword, term or phrase to describe the Public Service."@en;
  rdfs:label "keyword"@en .

dct:language a owl:ObjectProperty;
  rdfs:comment "The language(s) in which the Public Service is available."@en, "The language(s) in which the Rule is available."@en,
    "The language(s) in which the Evidence must be provided."@en, "The language(s) in which the Output is available."@en;
  rdfs:label "language"@en;
  skos:scopeNote """This could be one language or multiple languages, for instance in countries with more than one official language.

The recommended controlled vocabularies for this property is the <a href=\"https://op.europa.eu/en/web/eu-vocabularies/dataset/-/resource?uri=http://publications.europa.eu/resource/dataset/language\">Language</a> Authority Table of the Publications Office."""@en,
    "This could be one or multiple languages, for instance in countries with more than one official language. The recommended controlled vocabularies for this property is the <a href=\" https://op.europa.eu/en/web/eu-vocabularies/concept-scheme/-/resource?uri=http://publications.europa.eu/resource/authority/language\">Language</a> Authority Table of the Publications Office."@en,
    "The recommended controlled vocabularies for this property is the <a href=\"https://op.europa.eu/en/web/eu-vocabularies/dataset/-/resource?uri=http://publications.europa.eu/resource/dataset/language\">Language</a> Authority Table of the Publications Office."@en .

dct:title a owl:DatatypeProperty;
  rdfs:comment "The official Name of the Public Service."@en, "The Name of the Rule."@en,
    "The Name (or title) of the Event."@en, "The official Name of the piece of Evidence."@en,
    "The official Name of the Output."@en, "Name of the Requirement."@en, "The Name of the Service Concession Contract."@en,
    "A name given to the Dataset."@en, "The noun given to the Agent."@en;
  rdfs:label "name"@en, "title"@en;
  skos:scopeNote "This property can be repeated for parallel language versions of the name."@en .

cv:processingTime a owl:DatatypeProperty;
  rdfs:comment "The (estimated) time needed for executing a Public Service. The actual information is provided using the ISO8601 syntax for durations."@en,
    "The (estimated) time needed for executing a Public Service which may depend on the Channel chosen."@en;
  rdfs:label "processing time"@en;
  skos:scopeNote """Some examples are provided below:
Duration Syntax - Syntax
5 years - P5Y
1 month - P1M
3 days - P3D
2 days 4 hours - P2DT4H

Durations begin with an uppercase P followed by the number and the relevant designator, formally: P[n]Y[n]M[n]DT[n]H[n]M[n]S, where Y is for years, M for months etc. 

Note that days and times are separated by an uppercase T which also
disambiguates M as meaning month (P2M means 2 months) or minute (PT2M means 2 minutes). Durations may also be defined as a number of weeks so P4W means 4 weeks. A full explanation is provided in the <a href=\"https://en.wikipedia.org/wiki/ISO_8601#Durations\">Wikipedia page</a> that references the official <a href=\"https://www.iso.org/standard/40874.html\">ISO standard</a>.

This approach is consistent with both schema.org and the W3C OWL Time Ontology."""@en,
    "The actual information is provided using the ISO8601 syntax for durations."@en .

cv:sector a owl:ObjectProperty;
  rdfs:comment "The industry or sector a Public Service relates to, or is intended for."@en;
  rdfs:label "sector"@en;
  skos:scopeNote "For example: environment, safety, housing. Note that a single Public Service may relate to multiple sectors. The possible values for this property are provided as a controlled vocabulary. The possible values for this property are described in the controlled vocabulary <a href=\" https://op.europa.eu/en/web/eu-vocabularies/concept-scheme/-/resource?uri=http://publications.europa.eu/resource/authority/data-theme\">Data theme</a> Authority Table of the Publications Office."@en .

dct:spatial a owl:ObjectProperty;
  rdfs:comment "A Public Service is likely to be available only within a given area, typically the area covered by a particular public authority."@en,
    "It links an Organization to the Administrative Region(s) that it covers."@en;
  rdfs:label "spatial"@en;
  skos:scopeNote """A common usage of the spatial property will be to define the Administrative Territorial Unit(s) - typically a country or region - in which a Public Service is available. The Publications Office of the European Union offers <a href=\"https://op.europa.eu/en/web/eu-vocabularies/dataset/-/resource?uri=http://publications.europa.eu/resource/dataset/atu\">a URI set</a> that is suitable for this purpose. In case the ATU code list is not suitable, <a href=\"https://op.europa.eu/en/web/eu-vocabularies/dataset/-/resource?uri=http://publications.europa.eu/resource/dataset/nuts\">NUTS</a> or <a href=\"https://ec.europa.eu/eurostat/web/nuts/local-administrative-units\">LAU</a>, <a href=\"https://op.europa.eu/en/web/eu-vocabularies/dataset/-/resource?uri=http://publications.europa.eu/resource/dataset/place\">NAL Place</a> or <a href=\"http://www.geonames.org\">Geonames</a> are recommended to use, in that order. If those are still not sufficient, we recommend to define your own code list.

N.B. The spatial restriction is not meant to be used to describe eligibility or the speed of operation of the service. These aspects will be covered by the Criterion class."""@en,
    """The value of the properly should be the URI of the region as defined in an authoritative list of regions. In Europe, this is likely to be the Administrative Territorial Units Named Authority List maintained by the Publications Office's Metadata Registry.
<br/><br/>
The ATU list does not include a geometry. That is, the territory is only identified by its name not its spatial coordinates. This is likely to be the case for similar lists. If geometries are available for the Public Organization's territory, they can be linked from the territorial unit using the Core Location Vocabulary's locn:geometry property."""@en .

adms:status a owl:ObjectProperty;
  rdfs:comment "It indicates whether a Public Service is active, inactive, under development etc. according to a controlled vocabulary."@en;
  rdfs:label "status"@en .

cv:thematicArea a owl:ObjectProperty;
  rdfs:comment "The Thematic Area of a Public Service."@en;
  rdfs:label "thematic area"@en;
  skos:scopeNote "For example: social protection, health, recreation, culture and religion, family, traveling economic affairs, tax, staff, environment, etc."@en .

cv:contactPoint a owl:ObjectProperty;
  rdfs:comment "The main contact information of the resource."@en;
  rdfs:label "contact point"@en;
  skos:scopeNote "Note that the contact information should be relevant to the Public Service which may not be the same as contact information for the Competent Authority or any Participant."@en .

<http://purl.org/vocab/cpsv#follows> a owl:ObjectProperty;
  rdfs:comment "It links a Public Service to the Rule(s) under which it operates."@en;
  rdfs:label "follows"@en;
  skos:scopeNote "The definition of the Rule class is very broad. In a typical case, the competent authority that provides the public service will also define the rules that will implement its own policies. The CPSV-AP is flexible to allow for significant variation in such a scenario."@en .

cv:hasChannel a owl:ObjectProperty;
  rdfs:comment "It links the Public Service to any Channel through which an Agent provides, uses or otherwise interacts with the Public Service, such as an online service, phone number or office."@en;
  rdfs:label "has channel"@en .

cv:hasCompetentAuthority a owl:ObjectProperty;
  rdfs:comment "It links a Public Service to a Public Organization, which is the responsible Agent for the delivery of the Public Service."@en;
  rdfs:label "has competent authority"@en;
  skos:scopeNote "Whether the particular Public Organization provides the public service directly or outsources it is not relevant. The Public Organization that is the Competent Authority of the service is the one that is ultimately responsible for managing and providing the public service. The term Competent Authority is defined in the Services Directive (2006/123/EC) in the following way: \"Any body or authority which has a supervisory or regulatory role in a Member State in relation to service activities, including, in particular, administrative authorities, including courts acting as such, professional bodies, and those professional associations or other professional organisations which, in the exercise of their legal autonomy, regulate in a collective manner access to service activities or the exercise thereof\"."@en .

cv:hasCost a owl:ObjectProperty;
  rdfs:comment "It indicates the costs related to the execution of a Public Service for the citizen or business related to the execution of the particular Public Service."@en;
  rdfs:label "has cost"@en;
  skos:scopeNote "Where the cost varies depending on the channel through which the service is accessed, it can be linked to the channel using the If Accessed Through relationship."@en .

<http://purl.org/vocab/cpsv#hasInput> a owl:ObjectProperty;
  rdfs:comment "It links a Public Service to one or more instances of the Evidence class."@en,
    "The property links a Public Service directly to one or more pieces of Evidence."@en;
  rdfs:label "has input"@en;
  skos:scopeNote "A specific Public Service may require the presence of certain pieces of Evidence in order to be delivered. If the evidence required to make use of a service varies according to the channel through which it is accessed, then Has Input should be at the level of the Channel."@en,
    "In the majority of cases, the evidence required to use a Public Service will be independent of the channel through which the service is accessed. The Has Input property should normally be used to link a Public Service directly to one or more pieces of Evidence. However, where the type of Evidence required varies according to the channel used to access the Public Service, then the Has Input property may be used at the Channel level. For example, a digital signature may be required for an online channel, whereas a physical signature may be required for a face to face service provision."@en .

cv:hasInputType a owl:ObjectProperty;
  rdfs:comment "It links a Public Service to one or more instances of the EvidenceType class."@en;
  rdfs:label "has input type"@en .

cv:hasLegalResource a owl:ObjectProperty;
  rdfs:comment "It indicates the Legal Resource (e.g. legislation) to which the Public Service relates, operates or has its legal basis."@en;
  rdfs:label "has legal resource"@en .

cv:hasParticipation a owl:ObjectProperty;
  rdfs:comment "The way how a resource is organized."@en;
  rdfs:label "has participation"@en;
  skos:scopeNote "The Participation class facilitates the detailed description of how an Agent participates in or interacts with a Public Service and may include temporal and spatial information."@en .

cv:holdsRequirement a owl:ObjectProperty;
  rdfs:comment "It links a Public Service to a class that describes the Requirement."@en;
  rdfs:label "holds requirement"@en;
  skos:scopeNote "Usage: It describes the needing or using the service, such as residency in a given location, being over a certain age etc. The Requirement class is defined in the Core Criterion and Core Evidence Vocabulary."@en .

cv:isClassifiedBy a owl:ObjectProperty;
  rdfs:comment "It allows to classify the Public Service with any Concept other than those already foreseen and defined explicitly in the CPSV-AP (Thematic Area, Sector, etc.)."@en;
  rdfs:label "is classified by"@en;
  skos:scopeNote """It is a generic property which can be further specialised to make the classification explicit, for instance for classifying public services according level of digitisation,
type of audience, etc. The Concept is at its turn related to a Collection, which groups the different concepts into a controlled vocabulary."""@en .

dct:isPartOf a owl:ObjectProperty;
  rdfs:comment "A related resource in which the described resource is physically or logically included."@en;
  rdfs:label "is part of"@en;
  skos:scopeNote "It links a Public Service to the Dataset(s) in which it is being described."@en .

cv:isGroupedBy a owl:ObjectProperty;
  rdfs:comment "It links the Public Service to the Event class."@en;
  rdfs:label "is grouped by"@en;
  skos:scopeNote "Several Public Services may be associated with a particular Event and, likewise, the same Public Service may be associated with several different Events."@en .

<http://purl.org/vocab/cpsv#produces> a owl:ObjectProperty;
  rdfs:comment "It links a Public Service to one or more instances of the Output class, describing the actual result of executing a given Public Service."@en;
  rdfs:label "produces"@en;
  skos:scopeNote "Outputs can be any resource, for instance a document, artefact or anything else being produced as a result of executing the Public Service."@en .

cv:relatedService a owl:ObjectProperty;
  rdfs:comment "A Public Service related to the particular instance of the Public Service class."@en;
  rdfs:label "related service"@en;
  skos:scopeNote "This property is a sub-property of dct:relation."@en;
  rdfs:subPropertyOf dct:relation .

dct:requires a owl:ObjectProperty;
  rdfs:comment "The way a Public Service makes use of other Public Services."@en;
  rdfs:label "requires"@en;
  skos:scopeNote "One Public Service may require, or in some way make use of, the output of one or several other Public Services. In this case, for a Public Service to be executed, another Public Service must be executed beforehand. The nature of the requirement will be described in the associated Rule or Evidence."@en .

<http://purl.org/vocab/cpsv#Rule> a owl:Class;
  rdfs:comment "The Rule class represents a document that sets out the specific rules, guidelines or procedures that the Public Service follows."@en;
  rdfs:label "Rule"@en;
  skos:scopeNote "It includes the terms of service, licence, and authentication requirements of the Public Service. Instances of the Rule class are FRBR Expressions, that is, a concrete expression such as a document, of the more abstract concept of the rules themselves. The CPSV-AP does not envisage instances of the Rule class as machine-readable business rules. Detailed modelling of the rules related to Public Services is out of scope of the CPSV-AP."@en .

<http://purl.org/vocab/cpsv#implements> a owl:ObjectProperty;
  rdfs:comment """It links a Rule to relevant legislation or policy documents i.e.
the Legal Resource under which the Rules are being defined."""@en;
  rdfs:label "implements"@en .

cv:BusinessEvent a owl:Class;
  rdfs:comment "A Business Event is a specific situation or event in the lifecycle of a business that fulfils one or more needs or (legal) obligations of that business at this specific point in time."@en;
  rdfs:label "Business Event"@en;
  skos:scopeNote "A Business Event requires a set of public services to be delivered and consumed in order for the associated business need(s) or obligation(s) to be fulfilled. Business Events are defined within the context of a particular Member State. In other words, a Business Event groups together a number of public services that need to be delivered for completing that particular event."@en;
  rdfs:subClassOf cv:Event .

cv:Channel a owl:Class;
  rdfs:comment "A medium through which an Agent provides, uses or interacts in another way with a Public Service."@en;
  rdfs:label "Channel"@en;
  skos:scopeNote "Typical examples include online services, phone, walk-in centres etc."@en .

cv:specialOpeningHoursSpecification a owl:ObjectProperty;
  rdfs:comment "A time during which the resource is not available."@en;
  rdfs:label "availability restriction"@en;
  skos:scopeNote """Like the Contact Point, a Channel may not be available at a certain time.
<br/><br/>
For a simple description of the time use the description property of TemporalEntity.
<br/><br/>
For more structured data use the model in Time Ontology, see an <a href=\"https://www.w3.org/TR/owl-time/#dtd-vs-dt\">example</a>."""@en,
    """For a simple description of the time use the description property of TemporalEntity.

For more structured data use the model in Time Ontology, see an <a href=\"https://www.w3.org/TR/owl-time/#dtd-vs-dt\">example</a>."""@en .

cv:openingHours a owl:ObjectProperty;
  rdfs:comment "A time at which the resource is normally available."@en, "The time at which the Contact Point is normally available."@en;
  rdfs:label "opening hours"@en;
  skos:scopeNote """Like the Contact Point, a Channel may be available at a certain time.
<br/><br/>
For a simple description of the time use the description property of TemporalEntity.
<br/><br/>
For more structured data use the model in Time Ontology, see an <a href=\"https://www.w3.org/TR/owl-time/#dtd-vs-dt\">example</a>."""@en,
    """For a simple description of the time use the description property of TemporalEntity.

For more structured data use the model in Time Ontology, see an <a href=\"https://www.w3.org/TR/owl-time/#dtd-vs-dt\">example</a>. This relation can be used to indicate exceptional closures such as being closed on public holidays."""@en .

cv:ownedBy a owl:ObjectProperty;
  rdfs:comment "The owner of a specific Channel through which a Public Service is being delivered."@en;
  rdfs:label "owned by"@en .

cv:ContactPoint a owl:Class;
  rdfs:comment "Information (e.g. e-mail address, telephone number) of a person or department through which the user can get in touch with."@en;
  rdfs:label "Contact Point"@en;
  skos:scopeNote "Similarly to the Channel class, a Contact Point may have regular opening hours that are then overridden by, for example, public holidays, using the Temporal Entity class."@en .

cv:contactPage a owl:ObjectProperty;
  rdfs:comment "A web page that could be used to reach out the Contact Point."@en;
  rdfs:label "contact page"@en .

cv:email a owl:DatatypeProperty;
  rdfs:comment "An electronic address through which the Contact Point can be contacted."@en;
  rdfs:label "has email"@en .

cv:telephone a owl:DatatypeProperty;
  rdfs:comment "A telephone number through which the Contact Point can be contacted."@en;
  rdfs:label "has telephone"@en .

cv:Cost a owl:Class;
  rdfs:comment "The Cost class represents any costs related to the execution of a Public Service that the Agent consuming it needs to pay."@en;
  rdfs:label "Cost"@en .

cv:currency a owl:ObjectProperty;
  rdfs:comment "The currency in which the Cost needs to be paid and the value of the Cost is expressed."@en;
  rdfs:label "currency"@en;
  skos:scopeNote """The possible values for this property are described in the controlled vocabulary 
<a href=\"https://op.europa.eu/en/web/eu-vocabularies/concept-scheme/-/resource?uri=http://publications.europa.eu/resource/authority/currency\">Currency</a> Authority Table of Publications Office."""@en .

cv:hasValue a owl:DatatypeProperty;
  rdfs:comment "A numeric value indicating the amount of the Cost."@en;
  rdfs:label "has value"@en .

cv:ifAccessedThrough a owl:ObjectProperty;
  rdfs:comment "The costs created by the use of different Channels."@en;
  rdfs:label "if accessed through"@en;
  skos:scopeNote "For example, if accessed through an online service cf. accessed at a physical location, the cost can be linked to the channel using the If Accessed Through property."@en .

cv:isDefinedBy a owl:ObjectProperty;
  rdfs:comment "It links the Cost class to one or more instances of the Public Organization class."@en;
  rdfs:label "is defined by"@en;
  skos:scopeNote "This property indicates which Public Organization is the Competent Authority for defining the costs associated with the delivery of a particular Public Service."@en .

cv:Event a owl:Class;
  rdfs:comment "This class represents an event that can be of any type that triggers, makes use of, or in some way is related to, a Public Service."@en;
  rdfs:label "Event"@en;
  skos:scopeNote "It is not expected to be used directly, rather, one or other of its subclasses should be used. The properties of the class are, of course, inherited by those subclasses. The Event class is used as a hook either to a single related Public Service, such as diagnosis of illness being related to application for sickness benefit; or to a group of Public Services, such as all those related to the establishment of a new business."@en .

cv:hasRelatedService a owl:ObjectProperty;
  rdfs:comment "The Public Service related to the Event."@en;
  rdfs:label "has related service"@en;
  skos:scopeNote "This property is a sub-property of dct:relation."@en;
  rdfs:subPropertyOf dct:relation .

cv:Evidence a owl:Class;
  rdfs:comment "The Evidence class is defined in the Core Criterion and Core Evidence vocabulary (CCCEV) as any resource that can prove that a specific requirement is met."@en;
  rdfs:label "Evidence"@en;
  skos:scopeNote """Although the wording of the definition is different, the semantics are an exact match for CPSV's Input class which it replaces.

Evidence can be any resource - document, artefact - anything needed for executing the Public Service. In the context of Public Services, Evidence is usually administrative documents or completed application forms. A specific Public Service may require the presence of certain Evidence or combinations of Evidence in order to be delivered.

In some cases, the Output of one service will be Evidence for another service. Such relationships should be described in the associated Rule(s)."""@en .

foaf:page a owl:ObjectProperty;
  rdfs:comment "The documentation that contains information."@en;
  rdfs:label "related documentation"@en;
  skos:scopeNote "For instance, a particular template for an administrative document, an application or a guide on formatting the Evidence."@en .

dct:conformsTo a owl:ObjectProperty;
  rdfs:comment "Evidence Type that specifies characteristics of the Evidence."@en;
  rdfs:label "is conformant to"@en;
  skos:scopeNote "Examples of characteristics could be the layout or the configuration of the Evidence."@en .

cv:supportsRequirement a owl:ObjectProperty;
  rdfs:comment "Requirement for which the Evidence provides proof."@en;
  rdfs:label "supports requirement"@en .

cv:EvidenceType a owl:Class;
  rdfs:comment "Information about the characteristics of an Evidence."@en;
  rdfs:label "Evidence Type"@en;
  skos:scopeNote "The Evidence Type and the characteristics it describes are not concrete individual responses to a Requirement (i.e. Evidence), but descriptions about the desired form, content, source and/or other characteristics that an actual response should have and provide (e.g. membership of a class of Evidences)."@en .

cv:evidenceTypeClassification a owl:ObjectProperty;
  rdfs:comment "Category to which the Evidence Type belongs."@en;
  rdfs:label "evidence type classification"@en;
  skos:scopeNote "The categories agreed are left open but could for example specify the layout and content expected for an Evidence. An example could be id cards."@en .

cv:LifeEvent a owl:Class;
  rdfs:comment "The Life Event class represents an important event or situation in a citizen's life where public services are required."@en;
  rdfs:label "Life Event"@en;
  skos:scopeNote "Note on the scope: an individual will encounter any number of 'events'; in the general sense of the word. In the context of the CPSV-AP, the Life Event class only represents an event to which a Public Service is related. For example, a couple becoming engaged is not a CPSV-AP Life Event, getting married is, since only the latter has any relevance to public services."@en;
  rdfs:subClassOf cv:Event .

cv:Output a owl:Class;
  rdfs:comment "An output can be any resource - document, artefact - anything produced by the Public Service. In the context of a Public Service, the output provides an official document or other artefact of the Competent Authority (Public Organization) that permits/authorises/entitles an Agent to (do) something."@en;
  rdfs:label "Output"@en;
  skos:scopeNote "In some cases, the Output of one Public Service will be used as evidence to fulfil a requirement of another Public Service. Such relationships should be described in the associated Rule(s)."@en .

cv:Participation a owl:Class;
  rdfs:comment "The Participation class allows to define roles within a certain context."@en;
  rdfs:label "Participation"@en;
  skos:scopeNote """The CPSV-AP recognises a common role connected with public services, i.e. the Competent Authority.
<br/><br/>
This simple structure does not allow statements to be made about those participants, such as the start and end date of a contract, nor does it support the inclusion of other roles. The Participation class supports this extra complexity if required, for instance, the description of a service user or a service provider. The model is consistent with the CPOV which in turn is based on the W3C Organization Ontology that supports the common cases simply but allows the complex cases where necessary. The Participation class can be mapped to the Organization Ontology&#39;s Membership class that allows more complex relationships and richer metadata to be applied to a role filled by a given Agent."""@en .

cv:role a owl:ObjectProperty;
  rdfs:comment "The function of an Agent within a Participation."@en;
  rdfs:label "role"@en;
  skos:scopeNote """This should be provided using a controlled vocabulary.
Since this is an extension mechanism for the CSPV-AP, the controlled vocabulary should be decided to suit local implementations."""@en .

cv:hasParticipant a owl:ObjectProperty;
  rdfs:comment "The Agent involved in the Participation."@en;
  rdfs:label "has participant"@en .

cv:PublicOrganisation a owl:Class;
  rdfs:comment "An Organization that is defined as being part of the public sector by a legal framework at any level."@en;
  rdfs:label "Public Organization"@en;
  skos:scopeNote """Organizations which exist to provide services for its citizens and companies are called Public Organizations. The Public Organization class represents the organization. One organization may comprise several sub-organizations and any organization may have one or more organizational units. Each of these is described using the same properties and relationships.
<br/><br/>
This definition is consistent with the more detailed definition of a \"public sector body\" as given in the PSI Directive: \"the State, regional or local authorities, bodies governed by public law and associations formed by one or several such authorities or one or several such bodies governed by public law\". It further defines a body governed by public law as any body \"(a) established for the specific purpose of meeting needs in the general interest, not having an industrial or commercial character; and (b) having legal personality; and (c) financed, for the most part by the State, or regional or local authorities, or other bodies governed by public law; or subject to management supervision by those bodies; or having an administrative, managerial or supervisory board, more than half of whose members are appointed by the State, regional or local authorities or by other bodies governed by public law\"."""@en;
  rdfs:subClassOf org:Organization .

skos:prefLabel a owl:DatatypeProperty;
  rdfs:comment "A preferred label is used to provide the primary, legally recognised name of the Public Organization, as defined in the ORG Ontology."@en;
  rdfs:label "preferred label"@en;
  skos:scopeNote "Refers to the official or legal name of a Public Organization. An organization may only have one such name in any given language. Primary names may be provided in multiple languages with multiple instances of the preferred label property. This allowed in SKOS for skos:prefLabel, see <a href=\"https://www.w3.org/TR/skos-reference/#L1567\">integrity conditions and subsequent example</a>."@en .

cv:Requirement a owl:Class;
  rdfs:comment "Condition or prerequisite that is to be proven by Evidence."@en;
  rdfs:label "Requirement"@en;
  skos:scopeNote """Not all public services are needed or are used by everyone. For example, the visa service operated by European countries is not needed by European citizens but is needed by some citizens from elsewhere, or public services offering unemployment benefits and grants are targeting specific societal groups. The CPSV-AP reuses the Core Criterion and Core Evidence Vocabulary for this class.

Requirement is a generic class representing any type of prerequisite that may be desired, needed or imposed as an obligation. CCCEV recommends to not use the Requirement class directly, but rather a more semantically-enriched subclass such as Criterion, Information Requirement or Constraint. Also note that the Requirement class is specified at a more abstract level and is not to be used as the instantiation of a Requirement for a specific Agent.
To illustrate the notion: the European Directive on services in the internal market defines requirement as any obligation, prohibition, condition or limit provided for in the laws, regulations or administrative provisions of the Member States or in consequence of case-law, administrative practice, the rules of professional bodies, or the collective rules of professional associations or other professional organisations, adopted in the exercise of their legal autonomy."""@en .

cv:fulfils a owl:ObjectProperty;
  rdfs:comment "The Rules that the requiremens fulfils."@en;
  rdfs:label "fulfils"@en .

cv:hasSupportingEvidence a owl:ObjectProperty;
  rdfs:comment "Evidence that supplies information, proof or support for the Requirement."@en;
  rdfs:label "has supporting evidence"@en .

cv:ServiceConcessionContract a owl:Class;
  rdfs:comment "Concessions are contracts for pecuniary interest by means of which one or more contracting authorities or contracting entities entrusts the execution of works, or the provision and the management of services, to one or more economic operators."@en;
  rdfs:label "Service Concession Contract"@en;
  skos:scopeNote """The object of such contracts is the procurement of works or services by means of a concession, the consideration of which consists in the right to exploit the works or services or in that right together with payment. Such contracts may, but do not necessarily, involve a transfer of ownership to contracting authorities or contracting entities, but contracting authorities or contracting entities always obtain the benefits of the works or services in
question. The definition comes from the Directive <a href=\"https://eur-lex.europa.eu/legal-content/EN/TXT/HTML/?uri=CELEX:32014L0023&from=EN\">2014/23/EU</a>."""@en;
  rdfs:subClassOf <http://data.europa.eu/a4g/ontology#ConcessionContract> .

cv:establishedUnder a owl:ObjectProperty;
  rdfs:comment """It links a Service Concession Contract to relevant legislation or policy documents i.e.
the Legal Resource under which the Service Concession Contracts are being defined."""@en;
  rdfs:label "established under"@en .

cv:hasContractingAuthority a owl:ObjectProperty;
  rdfs:comment "It links a Service Concession Contract with the Contracting Authority which is ultimately responsible for a public service."@en;
  rdfs:label "has contracting authority"@en .

cv:hasEconomicOperator a owl:ObjectProperty;
  rdfs:comment "It links a Service Concession Contract with the Economic Operator in charge for the provision and the management of public services."@en;
  rdfs:label "has economic operator"@en .

dcat:Dataset a owl:Class;
  rdfs:comment "A collection of data, published or curated by a single agent, and available for access or download in one or more representations."@en;
  rdfs:label "Dataset"@en;
  skos:scopeNote "This class represents a collection of metadata and where they can be found. For instance, a dataset can be found on a regional public service portal and/or a national eGovernment portal."@en .

dcat:landingPage a owl:ObjectProperty;
  rdfs:comment "A web page that provides access to the Dataset, its Distributions and/or additional information."@en;
  rdfs:label "landing page"@en;
  skos:scopeNote "It is intended to point to a landing page at the original data provider, not to a page on a site of a third party, such as an aggregator."@en .

dct:hasPart a owl:ObjectProperty;
  rdfs:comment "It links a Dataset to the Public Service."@en;
  rdfs:label "has part"@en .

dct:publisher a owl:ObjectProperty;
  rdfs:comment "The Publisher of the Dataset, i.e. an entity (organisation) responsible for making the Dataset available."@en;
  rdfs:label "publisher"@en .

<http://data.europa.eu/eli/ontology#LegalResource> a owl:Class;
  rdfs:comment "This class represents the legislation, policy or policies that lie behind the Rules that govern the service."@en;
  rdfs:label "Legal Resource"@en;
  skos:scopeNote "The definition and properties of the Legal Resource class in the CPSV-AP are aligned with the ontology included in \"Council conclusions inviting the introduction of the European Legislation Identifier (ELI)\". For describing the attributes of a Legal Resource (labels, preferred labels, alternative labels, definition, etc.) we refer to the ELI ontology."@en .

dct:relation a owl:ObjectProperty;
  rdfs:comment "Another instance of the Legal Resource class that is related to the particular Legal Resource being described."@en;
  rdfs:label "related"@en .

<http://data.europa.eu/a4g/ontology#ConcessionContract> a owl:Class;
  rdfs:comment "A contract between one or more buyers and one or more economic operators giving the right to the economic operators to exploit the rights foreseen in the contract which may include the receipt of payments."@en;
  rdfs:label "Concession Contract"@en .

foaf:Agent a owl:Class;
  rdfs:comment "The Agent class is any resource that acts or has the power to act. This includes people, organisations and groups. The Public Organization class, defined in the Core Public Organisation Vocabulary, is a notable subclass of Agent."@en;
  rdfs:label "Agent"@en .

<http://www.w3.org/ns/locn#address> a owl:ObjectProperty;
  rdfs:comment "An Address related to an Agent. Asserting the address relationship implies that the Agent has an Address."@en;
  rdfs:label "address"@en .

cv:participates a owl:ObjectProperty;
  rdfs:comment "The participation in which an Agent is involved."@en;
  rdfs:label "participates"@en;
  skos:scopeNote "The Participation class facilitates the detailed description of how an Agent participates in or interacts with a Public Service and may include temporal and spatial information."@en .

<http://www.w3.org/ns/locn#Address> a owl:Class;
  rdfs:comment "A spatial object that in a human-readable way identifies a fixed location."@en;
  rdfs:label "Address"@en;
  skos:scopeNote """<p>
An \"address representation\" as conceptually defined by the <a href=\"https://inspire-regadmin.jrc.ec.europa.eu/dataspecification/ScopeObjectDetail.action?objectDetailId=9353
\">INSPIRE Address Representation data type</a>: \"Representation of an address spatial object for use in external application schemas that need to include the basic, address information in a readable way.\"
</p></br>

<p>
The representation of Addresses varies widely from one country's postal system to another. Even within countries, there are almost always examples of Addresses that do not conform to the stated national standard. However, <a href=\"https://www.iso.org/standard/61710.html\">ISO 19160-1</a> provides a method through which different Addresses can be converted from one conceptual model to another.
</p></br>

<p>
This specification was heavily based on the INSPIRE Address Representation data type. It is noteworthy that if an Address is provided using the detailed breakdown suggested by the properties for this class, then it will be INSPIRE-conformant. To this very granular set of
properties, we add two further properties:
<ul>
 <li>- full address (the complete address as a formatted string)</li>
 <li>- addressID (a unique identifier for the address)</li>
</ul>
The first of these allows publishers to simply provide the complete Address as one string, with or without formatting. This is analogous to <a href=\"https://www.w3.org/TR/vcard-rdf/#d4e953\">vCard's label property</a>.
</p></br>

<p>
The addressID is part of the INSPIRE guidelines and provides a hook that can be used to link the Address to an alternative representation, such as vCard or OASIS xAL.
</p></br>

This class belongs to <a href=\"https://semiceu.github.io/Core-Location-Vocabulary/releases/2.00/#Address\">Core Location Vocabulary</a>"""@en .

<http://www.w3.org/ns/locn#addressArea> a owl:DatatypeProperty;
  rdfs:comment "The name of a geographic area that groups Addresses."@en;
  rdfs:label "address area"@en;
  skos:scopeNote "This would typically be part of a city, a neighbourhood or village, e.g. Montmartre. Address area is not an administrative unit."@en .

<http://www.w3.org/ns/locn#addressId> a owl:DatatypeProperty;
  rdfs:comment "A globally unique identifier for each instance of an Address."@en;
  rdfs:label "address ID"@en;
  skos:scopeNote """The concept of adding a globally unique identifier for each instance of an address is a crucial part of the INSPIRE data spec. A number of EU countries have already implemented an ID (a UUID) in their Address Register/gazetteer, among them Denmark. OASIS xAL also includes an address identifier. It is the address Identifier that allows an address to be represented in a format other than INSPIRE whilst remaining conformant to the Core Vocabulary.
<br/><br/>
The INSPIRE method of representing addresses is very detailed, designed primarily for use in databases of addresses. Whilst data that is published in full conformance with the INSPIRE data structure can be made available using the Core Location Vocabulary the reverse is not true since the Core Vocabulary allows much greater flexibility.
<br/><br/>
Many datasets that include address data as one piece of information about something else are likely to have that data in simpler formats. These might be tailored to the specific need of the dataset, follow a national norm, or make use of a standard like vCard.
<br/><br/>
To provide maximum flexibility in the Core Vocabulary, whilst remaining interoperable with INSPIRE Address Guidelines (which EU Member States are obliged to use), the Core Location Vocabulary provides the extra property of full address and makes use of INSPIRE's addressID."""@en .

<http://www.w3.org/ns/locn#adminUnitL1> a owl:DatatypeProperty;
  rdfs:comment "The name of the uppermost level of the address, almost always a country."@en;
  rdfs:label "administrative unit level 1"@en;
  skos:scopeNote "Best practice is to use the ISO 3166-1 code but if this is inappropriate for the context, country names should be provided in a consistent manner to reduce ambiguity. For example, either write 'France' or 'FRA' consistently throughout the dataset and avoid mixing the two. The <a href=\"https://op.europa.eu/en/web/eu-vocabularies/dataset/-/resource?uri=http://publications.europa.eu/resource/dataset/country\">Country controlled vocabulary</a> from the Publications Office can be reused for this."@en .

<http://www.w3.org/ns/locn#adminUnitL2> a owl:DatatypeProperty;
  rdfs:comment "The name of a secondary level/region of the address, usually a county, state or other such area that typically encompasses several localities."@en;
  rdfs:label "administrative unit level 2"@en;
  skos:scopeNote "Values could be a region or province, more granular than level 1."@en .

<http://www.w3.org/ns/locn#fullAddress> a owl:DatatypeProperty;
  rdfs:comment "The complete address written as a string."@en;
  rdfs:label "full address"@en;
  skos:scopeNote "Use of this property is not recommended as it will suffer any misunderstandings that might arise through the breaking up of an address into its component parts. This property is analogous to vCard's label property but with two important differences: (1) formatting is not assumed so that, unlike vCard label, it may not be suitable to print this on an address label, (2) vCard's label property has a domain of vCard Address; the fullAddress property has no such restriction. An example of a full address is \"Champ de Mars, 5 Avenue Anatole France, 75007 Paris, France\"."@en .

<http://www.w3.org/ns/locn#locatorDesignator> a owl:DatatypeProperty;
  rdfs:comment "A number or sequence of characters that uniquely identifies the locator within the relevant scope."@en;
  rdfs:label "locator designator"@en;
  skos:scopeNote "In simpler terms, this is the building number, apartment number, etc. For an address such as \"Flat 3, 17 Bridge Street\", the locator is \"flat 3, 17\"."@en .

<http://www.w3.org/ns/locn#locatorName> a owl:DatatypeProperty;
  rdfs:comment "Proper noun(s) applied to the real world entity identified by the locator."@en;
  rdfs:label "locator name"@en;
  skos:scopeNote """The locator name could be the name of the property or complex, of the building or part of the building, or it could be the name of a room inside a building.
<br/><br/>
The key difference between a locator and a locator name is that the latter is a proper name and is unlikely to include digits. For example, \"Shumann, Berlaymont\" is a meeting room within the European Commission headquarters for which locator name is more appropriate than locator."""@en .

<http://www.w3.org/ns/locn#poBox> a owl:DatatypeProperty;
  rdfs:comment "A location designator for a postal delivery point at a post office, usually a number."@en;
  rdfs:label "post office box"@en;
  skos:scopeNote "INSPIRE's name for this is \"postalDeliveryIdentifier\" for which it uses the locator designator property with a type attribute of that name. This vocabulary separates out the Post Office Box for greater independence of technology. An example post office box number is \"9383\"."@en .

<http://www.w3.org/ns/locn#postCode> a owl:DatatypeProperty;
  rdfs:comment "The code created and maintained for postal purposes to identify a subdivision of addresses and postal delivery points."@en;
  rdfs:label "post code"@en;
  skos:scopeNote "Post codes are common elements in many countries' postal address systems. One of the many post codes of Paris is for example \"75000\"."@en .

<http://www.w3.org/ns/locn#postName> a owl:DatatypeProperty;
  rdfs:comment "A name created and maintained for postal purposes to identify a subdivision of addresses and postal delivery points."@en;
  rdfs:label "post name"@en;
  skos:scopeNote "Usually a city, for example \"Paris\"."@en .

<http://www.w3.org/ns/locn#thoroughfare> a owl:DatatypeProperty;
  rdfs:comment "The name of a passage or way through from one location to another."@en;
  rdfs:label "thoroughfare"@en;
  skos:scopeNote "A thoroughfare is usually a street, but it might be a waterway or some other feature. For example, \"Avenue des Champs-lyses\"."@en .

org:Organization a owl:Class;
  rdfs:comment "A collection of people organized together into a community or other social, commercial or political structure. The group has some common purpose or reason for existence which goes beyond the set of people belonging to it and can act as an Agent. Organizations are often decomposable into hierarchical structures."@en;
  rdfs:label "Organization"@en;
  rdfs:subClassOf foaf:Agent .

skos:Collection a owl:Class;
  rdfs:comment "This class represent the way Concepts belong together. Thus, different concepts are grouped and define a controlled vocabulary."@en;
  rdfs:label "Collection"@en;
  skos:scopeNote "In this context, the CPSV-AP reuses the Collection class as defined in the SKOS Simple Knowledge Organization System. For describing the attributes of a Collection (labels, preferred labels, alternative labels, definition, etc.) we refer to SKOS."@en .

skos:member a owl:ObjectProperty;
  rdfs:comment "It indicates the Concepts that are part of the Collection."@en;
  rdfs:label "member"@en .

skos:Concept a owl:Class;
  rdfs:comment "This class represents any concept that can be used for classifying the Public Service and which relates to the Public Service through the property Is Classified By."@en;
  rdfs:label "Concept"@en;
  skos:scopeNote "This class has been added in the CPSV-AP to complement the need for adding other ways of classifying the Public Service, which have not been explicitly defined in the CPSV-AP. In this context, the CPSV-AP reuses the Concept class as defined in the SKOS Simple Knowledge Organization System. For describing the attributes of a Concept (labels, preferred labels, alternative labels, definition, etc.) we refer to SKOS. The Concept may or may not belong to (member) a certain Collection."@en .

<http://www.w3.org/2006/time#TemporalEntity> a owl:Class;
  rdfs:comment "A temporal interval or instant."@en;
  rdfs:label "Temporal Entity"@en .

cv:frequency a owl:ObjectProperty;
  rdfs:comment "The recurrence of an instant or period."@en;
  rdfs:label "frequency"@en;
  skos:scopeNote "It is recommended to use the frequency from an existing vocabulary like the <a href=\"https://op.europa.eu/en/web/eu-vocabularies/concept-scheme/-/resource?uri=http://publications.europa.eu/resource/authority/frequency\">Frequency</a> from the Publications Office."@en .
