@prefix : <http://data.europa.eu/m8g/cpsvap#> .
@prefix cv: <http://data.europa.eu/m8g/> .
@prefix dct: <http://purl.org/dc/terms/> .
@prefix eli: <http://data.europa.eu/eli/ontology#> .
@prefix org: <http://www.w3.org/ns/org#> .
@prefix owl: <http://www.w3.org/2002/07/owl#> .
@prefix rdf: <http://www.w3.org/1999/02/22-rdf-syntax-ns#> .
@prefix xml: <http://www.w3.org/XML/1998/namespace> .
@prefix xsd: <http://www.w3.org/2001/XMLSchema#> .
@prefix adms: <http://www.w3.org/ns/adms#> .
@prefix cpsv: <http://purl.org/vocab/cpsv#> .
@prefix dcat: <http://www.w3.org/ns/dcat#> .
@prefix foaf: <http://xmlns.com/foaf/0.1/> .
@prefix locn: <http://www.w3.org/ns/locn#> .
@prefix rdfs: <http://www.w3.org/2000/01/rdf-schema#> .
@prefix skos: <http://www.w3.org/2004/02/skos/core#> .
@prefix vann: <http://purl.org/vocab/vann/> .
@base <http://data.europa.eu/m8g/cpsvap> .

<http://data.europa.eu/m8g/cpsvap> rdf:type owl:Ontology ;
                                    dct:created "2018-07-09"^^xsd:date ;
                                    dct:creator <http://publications.europa.eu/resource/authority/corporate-body/DIGIT> ;
                                    dct:license <https://creativecommons.org/licenses/by-nc/4.0/> ;
                                    vann:preferredNamespacePrefix "cpsvap" ;
                                    owl:versionInfo "3.0.0" ;
                                    foaf:homepage <https://joinup.ec.europa.eu/asset/cpsv-ap/home> .

#################################################################
#    Annotation properties
#################################################################

###  http://purl.org/dc/terms/created
dct:created rdf:type owl:AnnotationProperty .


###  http://purl.org/dc/terms/creator
dct:creator rdf:type owl:AnnotationProperty .


###  http://purl.org/dc/terms/hasVersion
dct:hasVersion rdf:type owl:AnnotationProperty .


###  http://purl.org/dc/terms/license
dct:license rdf:type owl:AnnotationProperty .


###  http://purl.org/vocab/vann/preferredNamespacePrefix
vann:preferredNamespacePrefix rdf:type owl:AnnotationProperty .


###  http://purl.org/vocab/vann/usageNote
vann:usageNote rdf:type owl:AnnotationProperty .


###  http://xmlns.com/foaf/0.1/homepage
foaf:homepage rdf:type owl:AnnotationProperty .


#################################################################
#    Datatypes
#################################################################

###  http://www.w3.org/1999/02/22-rdf-syntax-ns#langString
rdf:langString rdf:type rdfs:Datatype .


###  http://www.w3.org/2001/XMLSchema#duration
xsd:duration rdf:type rdfs:Datatype .


#################################################################
#    Object Properties
#################################################################

###  http://data.europa.eu/m8g/contactPage
cv:contactPage rdf:type owl:ObjectProperty ;
               rdfs:range <http://xmlns.com/foaf/0.1/Document> ;
               rdfs:comment "Cardinality [0..*]. A contact form that could be used to reach out the contact point."@en ;
               rdfs:label "contact page"@en .


###  http://data.europa.eu/m8g/currency
cv:currency rdf:type owl:ObjectProperty ;
            rdfs:range skos:Concept ;
            vann:usageNote "The CPSV-AP v2.0 recommends to use as controlled vocabulary the European Publications Office's Currencies Named Authority List (NAL) (http://publications.europa.eu/mdr/authority/currency/index.html)."@en ;
            rdfs:comment "Cardinality [0..1]. This property represents the currency in which the Cost needs to be paid and the value of the Cost is expressed. The possible values for this property are described in a controlled vocabulary."@en ;
            rdfs:label "currency"@en .


###  http://data.europa.eu/m8g/hasChannel
cv:hasChannel rdf:type owl:ObjectProperty ;
              rdfs:range cv:Channel ;
              rdfs:comment "Cardinality [0..n]. This property links the Public Service to any Channel through which an Agent provides, uses or otherwise interacts with the Public Service, such as an online service, phone number or office."@en ;
              rdfs:label "has channel"@en .


###  http://data.europa.eu/m8g/hasCompetentAuthority
cv:hasCompetentAuthority rdf:type owl:ObjectProperty ;
                         rdfs:range cv:PublicOrganisation ;
                         rdfs:comment "Cardinality [1..n]. This property links a Public Service to a Public Organisation, which is the responsible Agent for the delivery of the Public Service. Whether the particular Public Organisation provides the public service directly or outsources it is not relevant. The Public Organisation that is the Competent Authority of the service is the one that is ultimately responsible for managing and providing the public service."@en ;
                         rdfs:label "has competent authority"@en .


###  http://data.europa.eu/m8g/hasContactPoint
cv:hasContactPoint rdf:type owl:ObjectProperty ;
                   rdfs:range cv:ContactPoint ;
                   rdfs:comment "Cardinality [0..n]. A contact point for the service is almost always helpful. The value of this property, the contact information itself, should be provided using VCard. Note that the contact information should be relevant to the Public Service which may not be the same as contact information for the Competent Authority or any Participant."@en ;
                   rdfs:label "has contact point"@en .


###  http://data.europa.eu/m8g/hasCost
cv:hasCost rdf:type owl:ObjectProperty ;
           rdfs:range cv:Cost ;
           rdfs:comment "Cardinality [0..n]. The Has Cost property links a Public Service to one or more instances of the Cost class. It indicates the costs related to the execution of a Public Service for the citizen or business related to the execution of the particular Public Service. Where the cost varies depending on the channel through which the service is accessed, it can be linked to the channel using the If Accessed Through relationship."@en ;
           rdfs:label "has cost"@en .


###  http://data.europa.eu/m8g/hasLegalResource
cv:hasLegalResource rdf:type owl:ObjectProperty ;
                    rdfs:range eli:LegalResource ;
                    rdfs:comment "Cardinality [0..n]. The Has Legal Resource property links a Public Service to a Legal Resource. It indicates the Legal Resource (e.g. legislation) to which the Public Service relates, operates or has its legal basis."@en ;
                    rdfs:label "has legal resource"@en .


###  http://data.europa.eu/m8g/hasParticipation
cv:hasParticipation rdf:type owl:ObjectProperty ;
                    rdfs:range cv:Participation ;
                    rdfs:comment "Cardinality [0..n]. This property links a Public Service to the Participation class. The Participation class facilitates the detailed description of how an Agent participates in or interacts with a Public Service and may include temporal and spatial information."@en ;
                    rdfs:label "has participation"@en .


###  http://data.europa.eu/m8g/holdsRequirement
cv:holdsRequirement rdf:type owl:ObjectProperty ;
                    rdfs:range cv:Requirement ;
                    rdfs:comment "Cardinality [0..n]. Links a Public Service to a class that describes the requirement for needing or using the service, such as residency in a given location, being over a certain age etc. The Requirement class is defined in the Core Criterion and Core Evidence Vocabulary"@en ;
                    rdfs:label "holds requirement"@en .


###  http://data.europa.eu/m8g/hoursAvailable
cv:hoursAvailable rdf:type owl:ObjectProperty ;
                  rdfs:range cv:OpeningHoursSpecification ;
                  rdfs:comment "Cardinality [0..1]. This property links a channel to information about when the channel is not available, overriding the general opening hours information. The details are provided using the Opening Hours Specification class."@en ,
                               "Cardinality [0..n]. This property links a channel to information about when the channel is not available, overriding the general opening hours information. The details are provided using the Opening Hours Specification class."@en ;
                  rdfs:label "availability restriction"@en .


###  http://data.europa.eu/m8g/ifAccessedThrough
cv:ifAccessedThrough rdf:type owl:ObjectProperty ;
                     rdfs:range cv:Channel ;
                     rdfs:comment "Cardinality [0..1]. Where the cost varies depending on the channel used, for example, if accessed through an online service cf. accessed at a physical location, the cost can be linked to the channel using the If Accessed Through property."@en ;
                     rdfs:label "if accessed through"@en .


###  http://data.europa.eu/m8g/isClassifiedBy
cv:isClassifiedBy rdf:type owl:ObjectProperty ;
                  rdfs:range skos:Concept ;
                  rdfs:comment "Cardinality [0..n]. The Is Classified By property allows to classify the Public Service with any Concept, other than those already foreseen and defined explicitely in the CPSV-AP (Thematic Area, Sector, …). It is a generic property which can be further specialised to make the classification explicit, for instance for classifying public services according level of digitisation, type of audience … The Concept is at its turn related to a Collection, which groups the different concepts into a controlled vocabulary."@en ;
                  rdfs:label "is classified by"@en .


###  http://data.europa.eu/m8g/isDefinedBy
cv:isDefinedBy rdf:type owl:ObjectProperty ;
               rdfs:range org:Organization ;
               rdfs:comment "Cardinality [0..n]. This property links the Cost class with one or more instances of the Public Organisation class. This property indicates which Public Organisation is the Competent Authority for defining the costs associated with the delivery of a particular Public Service."@en ;
               rdfs:label "is defined by"@en .


###  http://data.europa.eu/m8g/isDescribedAt
cv:isDescribedAt rdf:type owl:ObjectProperty ;
                 rdfs:range <https://www.w3.org/ns/dcat#Dataset> ;
                 rdfs:comment "Cardinality [0..n]. The Is Described At property links a Public Service to the dataset where it belongs to. It is used to track the metadata of the origin of the public service descriptions."@en ;
                 rdfs:label "is described at"@en .


###  http://data.europa.eu/m8g/isGroupedBy
cv:isGroupedBy rdf:type owl:ObjectProperty ;
               rdfs:range cv:Event ;
               rdfs:comment "Cardinality [0..n]. This property links the Public Service to the Event class. Several Public Services may be associated with a particular Event and, likewise, the same Public Service may be associated with several different Events."@en ;
               rdfs:label "is grouped by"@en .


###  http://data.europa.eu/m8g/ownedBy
cv:ownedBy rdf:type owl:ObjectProperty ;
           rdfs:range org:Organization ;
           rdfs:comment "Cardinality [0..n]. This property links the Channel class with one or more instances of the Public Organisation class. This property indicates the owner of a specific Channel through which a Public Service is being delivered."@en ;
           rdfs:label "owned by"@en .


###  http://data.europa.eu/m8g/playsRole
cv:playsRole rdf:type owl:ObjectProperty ;
             rdfs:range cv:Participation ;
             rdfs:comment "Cardinality [0..n]. This property links an Agent to the Participation class. The Participation class facilitates the detailed description of how an Agent participates in or interacts with a Public Service and may include temporal and spatial information."@en ;
             rdfs:label "plays role"@en .


###  http://data.europa.eu/m8g/role
cv:role rdf:type owl:ObjectProperty ;
        rdfs:range skos:Concept ;
        rdfs:comment "Cardinality [1..n]. Provides the role played. This should be provided using a controlled vocabulary. Since this is an extension mechanism for the CSPV-AP, the controlled vocabulary should be decided to suit local implementations"@en ;
        rdfs:label "role"@en .


###  http://data.europa.eu/m8g/sector
cv:sector rdf:type owl:ObjectProperty ;
          rdfs:range skos:Concept ;
          rdfs:comment "Cardinality [0..n]. This property represents the industry or sector a Public Service relates to, or is intended for. For example: environment, safety, housing. Note that a single Public Service may relate to multiple sectors. The possible values for this property are provided as a controlled vocabulary."@en ;
          rdfs:label "sector"@en .


###  http://data.europa.eu/m8g/thematicArea
cv:thematicArea rdf:type owl:ObjectProperty ;
                rdfs:range skos:Concept ;
                rdfs:comment "Cardinality [0..1]. Indicates whether a Public Service is active, inactive, under development etc. according to a controlled vocabulary."@en ;
                rdfs:label "thematicArea"@en .


###  http://purl.org/dc/terms/language
dct:language rdf:type owl:ObjectProperty ;
             rdfs:range <http://purl.org/dc/terms/LinguisticSystem> ;
             vann:usageNote "The recommended controlled vocabularies for this property is the Language Authority Table of the Publications Office (https://op.europa.eu/en/web/eu-vocabularies/dataset/-/resource?uri=http://publications.europa.eu/resource/dataset/language)"@en ;
             rdfs:comment "Cardinality [0..n]. Indicates the language(s) in which the Evidence must be provided."@en ,
                          "Cardinality [0..n]. This property represents the language(s) in which the Output is available. This could be one or multiple languages, for instance in countries with more than one official language."@en ,
                          "Cardinality [0..n]. This property represents the language(s) in which the Public Service is available. This could be one language or multiple languages, for instance in countries with more than one official language."@en ,
                          "Cardinality [0..n]. This property represents the language(s) in which the Rule is available. This could be one or multiple languages, for instance in countries with more than one official language."@en ;
             rdfs:label "language"@en .


###  http://purl.org/dc/terms/publisher
dct:publisher rdf:type owl:ObjectProperty ;
              rdfs:range foaf:Agent ;
              rdfs:comment "Cardinality [1..1]. This property represents the Publisher of the Public Service Dataset, i.e. an entity (organisation) responsible for making the Public Service Dataset available."@en ;
              rdfs:label "publisher"@en .


###  http://purl.org/dc/terms/relation
dct:relation rdf:type owl:ObjectProperty ;
             rdfs:range cpsv:PublicService ;
             rdfs:comment "Cardinality [0..n]. This property links an event directly to a public service that is related to it."@en ;
             rdfs:label "related service"@en .


###  http://purl.org/dc/terms/requires
dct:requires rdf:type owl:ObjectProperty ;
             rdfs:range cpsv:PublicService ;
             rdfs:comment "Cardinality [0..n]. One Public Service may require, or in some way make use of, the output of one or several other Public Services. In this case, for a Public Service to be executed, another Public Service must be executed beforehand. The nature of the requirement will be described in the associated Rule or Evidence."@en ;
             rdfs:label "requires"@en .


###  http://purl.org/dc/terms/spatial
dct:spatial rdf:type owl:ObjectProperty ;
            rdfs:range <http://purl.org/dc/terms/Location> ;
            vann:usageNote "A common usage of the spatial property will be to define the Administrative Territorial Unit(s) - typically a country or region - in which a Public Service is available. The Publications Office of the European Union offers URI set (https://op.europa.eu/en/web/eu-vocabularies/dataset/-/resource?uri=http://publications.europa.eu/resource/dataset/atu) that is suitable for this purpose, e.g. Malta is identified by http://publications.europa.eu/resource/authority/atu/MLT, West Flanders by http://publications.europa.eu/resource/authority/atu/BEL_PR_WVL and so on. In case the ATU code list is not suitable, NUTS (https://op.europa.eu/en/web/eu-vocabularies/dataset/-/resource?uri=http://publications.europa.eu/resource/dataset/nuts) or LAU (https://ec.europa.eu/eurostat/web/nuts/local-administrative-units), NAL Place (https://op.europa.eu/en/web/eu-vocabularies/dataset/-/resource?uri=http://publications.europa.eu/resource/dataset/place) or Geonames (http://www.geonames.org/) are recommended to use, in that order. If those are still not sufficient, we recommend to define your own code list. N.B. The spatial restriction is not meant to be used to describe eligibility or the speed of operation of the service. These aspects will be covered by the Criterion class."@en ,
                           "The value should be a URI from the Administrative Territorial Units (https://op.europa.eu/en/web/eu-vocabularies/dataset/-/resource?uri=http://publications.europa.eu/resource/dataset/atu) Authority Table maintained by the Publications Office."@en ;
            rdfs:comment "Cardinality [0..n]. A Public Service is likely to be available only within a given area, typically the area covered by a particular public authority."@en ,
                         "Cardinality [1..n]. A Public Organisation has to be associated to one or multiple locations."@en ;
            rdfs:label "spatial"@en .


###  http://purl.org/vocab/cpsv#follows
cpsv:follows rdf:type owl:ObjectProperty ;
             rdfs:range cpsv:Rule ;
             rdfs:comment "Cardinality [0..n]. The follows property links a Public Service to the Rule(s) under which it operates. The definition of the Rule class is very broad. In a typical case, the competent authority that provides the public service will also define the rules that will implement its own policies. The CPSV-AP is flexible to allow for significant variation in such a scenario."@en ;
             rdfs:label "follows"@en .


###  http://purl.org/vocab/cpsv#hasInput
cpsv:hasInput rdf:type owl:ObjectProperty ;
              rdfs:range cv:Evidence ;
              vann:usageNote "Cardinality [0..n]. The Has Input property links a Public Service to one or more instances of the Evidence class. A specific Public Service may require the presence of certain pieces of Evidence in order to be delivered. If the evidence required to make use of a service varies according to the channel through which it is accessed, then Has Input should be at the level of the Channel."@en ;
              rdfs:comment "Cardinality [0..n]. In the majority of cases, the evidence required to use a Public Service will be independent of the channel through which the service is accessed. The Has Input property should normally be used to link a Public Service directly to one or more pieces of Evidence. However, where the type of Evidence required varies according to the channel used to access the Public Service, then the Has Input property may be used at the Channel level. For example, a digital signature may be required for an online channel, whereas a physical signature may be required for a face to face service provision."@en ;
              rdfs:label "has input"@en .


###  http://purl.org/vocab/cpsv#implements
cpsv:implements rdf:type owl:ObjectProperty ;
                rdfs:range eli:LegalResource ;
                rdfs:comment "Cardinality [0..n]. The Implements property links a Rule to relevant legislation or policy documents i.e. the Formal Framework under which the Rules are being defined."@en ;
                rdfs:label "implements"@en .


###  http://purl.org/vocab/cpsv#produces
cpsv:produces rdf:type owl:ObjectProperty ;
              rdfs:range cv:Output ;
              rdfs:comment "Cardinality [0..n]. The Produces property links a Public Service to one or more instances of the Output class, describing the actual result of executing a given Public Service. Outputs can be any resource, for instance a document, artefact or anything else being produced as a result of executing the Public Service."@en ;
              rdfs:label "produces"@en .


###  http://www.w3.org/2004/02/skos/core#member
skos:member rdf:type owl:ObjectProperty ;
            rdfs:range skos:Concept ;
            rdfs:comment "Cardinality [0..n]. The Member property, as defined in SKOS, allows to indicate the Concepts that are part of a Collection."@en ;
            rdfs:label "member"@en .


###  http://www.w3.org/ns/adms#status
adms:status rdf:type owl:ObjectProperty ;
            rdfs:range skos:Concept ;
            rdfs:comment "Cardinality [0..1]. Indicates whether a Public Service is active, inactive, under development etc. according to a controlled vocabulary."@en ;
            rdfs:label "status"@en .


###  http://www.w3.org/ns/dcat#landingPage
dcat:landingPage rdf:type owl:ObjectProperty ;
                 rdfs:range <http://xmlns.com/foaf/0.1/Document> ;
                 vann:usageNote "It is intended to point to a landing page at the original data provider, not to a page on a site of a third party, such as an aggregator." ;
                 rdfs:comment "Cardinality [0..n]. This property refers to a web page that provides access to the Dataset, its Distributions and/or additional information."@en ;
                 rdfs:label "landing page"@en .


###  http://www.w3.org/ns/locn#address
locn:address rdf:type owl:ObjectProperty ;
             rdfs:range locn:Address ;
             rdfs:comment "Cardinality [0..1]. This property represents an Address related to an Agent. Asserting the address relationship implies that the Agent has an Address."@en ;
             rdfs:label "address"@en .


###  http://xmlns.com/foaf/0.1/page
foaf:page rdf:type owl:ObjectProperty ;
          rdfs:range <http://xmlns.com/foaf/0.1/Document> ;
          rdfs:comment "Cardinality [0..n]. This property represents documentation that contains information related to the Evidence, for instance a particular template for an administrative document, an application or a guide on formatting the Input."@en ;
          rdfs:label "related documentation"@en .


###  http://purl.org/dc/terms/hasPart
<http://purl.org/dc/terms/hasPart> rdf:type owl:ObjectProperty ;
                                    rdfs:range cpsv:PublicService ;
                                    rdfs:comment "Cardinality [0..n]. The has part property links a Public Service Dataset to the Public Service."@en ;
                                    rdfs:label "has part"@en .


###  http://purl.org/dc/terms/relation
<http://purl.org/dc/terms/relation> rdf:type owl:ObjectProperty ;
                                     rdfs:range eli:LegalResource ,
                                                cpsv:PublicService ;
                                     rdfs:comment "Cardinality [0..n]. This property represents a Public Service related to the particular instance of the Public Service class."@en ,
                                                  "Cardinality [0..n]. This property represents another instance of the Legal Resource class that is related to the particular Legal Resource being described."@en ;
                                     rdfs:label "related"@en .


###  http://purl.org/dc/terms/type
<http://purl.org/dc/terms/type> rdf:type owl:ObjectProperty ;
                                 rdfs:range skos:Concept ;
                                 vann:usageNote "Possible values of Output types are: Declaration, Physical object, Code, Financial obligation, Financial benefit, Recognition, Permit"@en ;
                                 rdfs:comment "Cardinality [0..1]. This property represents the type of Evidence as described in a controlled vocabulary."@en ,
                                              "Cardinality [0..1]. Type of Rule."@en ,
                                              "Cardinality [0..n]. The type property links an Event to a controlled vocabulary of event types and it is the nature of those controlled vocabularies that is the major difference between a business event, such as creating the business in the first place and a life event, such as the birth of a child."@en ,
                                              "Cardinality [0..n]. This property represents the Type of a Public Service as described in a controlled vocabulary. For the indicating the Type, we are referring to the functions of government to indicate the purpose of a government activity, which the public service is intended for."@en ,
                                              "Cardinality [0..n]. This property represents the type of Channel as defined in a controlled vocabulary."@en ,
                                              "Cardinality [0..n]. This property represents the type of Output as defined in a controlled vocabulary.."@en ,
                                              "Cardinality [0..n]. This property represents the type of Requirement as described in a controlled vocabulary."@en ;
                                 rdfs:label "Type"@en .


#################################################################
#    Data properties
#################################################################

###  http://data.europa.eu/m8g/email
cv:email rdf:type owl:DatatypeProperty ;
         rdfs:range rdf:langString ;
         rdfs:comment "Cardinality [0..n]. the email of the ContactPoint"@en ;
         rdfs:label "has email"@en .


###  http://data.europa.eu/m8g/hasValue
cv:hasValue rdf:type owl:DatatypeProperty ;
            rdfs:range xsd:double ;
            rdfs:comment "Cardinality [0..1]. This property represents a numeric value indicating the amount of the Cost."@en ;
            rdfs:label "has value"@en .


###  http://data.europa.eu/m8g/openingHours
cv:openingHours rdf:type owl:DatatypeProperty ;
                rdfs:range rdf:langString ;
                vann:usageNote "The value should follow the flexible format defined for schema.org's opening hours property. Following that structure, days of the week are represented by two letter codes (Mo,Tu, We, Th, Fr, Sa, Su). Lists should be comma separated (for example: Mo, We, Fr) and periods separated by a hyphen (for example: Mo-Fr). If it is appropriate to add opening hours then this follows the day so if a phone service is available 08:00-20:00 Monday to Saturday and 08:00-18:00 on Sundays that would be encoded as Mo-Sa 08:00-20:00, Su 08:00-18:00."@en ;
                rdfs:comment "Cardinality [0..n]. This property represents the normal opening hours of a channel."@en ;
                rdfs:label "opening hours"@en .


###  http://data.europa.eu/m8g/processingTime
cv:processingTime rdf:type owl:DatatypeProperty ;
                  rdfs:range xsd:duration ;
                  vann:usageNote "Some examples are provided below: Duration Syntax - Syntax 5 years - P5Y 1 month - P1M 3 days - P3D 2 days 4 hours - P2DT4H Durations begin with an uppercase P followed by the number and the relevant designator, formally: P[n]Y[n]M[n]DT[n]H[n]M[n]S, where Y is for years, M for months etc. Note that days and times are separated by an uppercase T which also disambiguates M as meaning month (P2M means 2 months) or minute (PT2M means 2 minutes). Durations may also be defined as a number of weeks so P4W means 4 weeks. A full explanation is provided in the Wikipedia page that references the official ISO standard. This approach is consistent with both schema.org and the W3C OWL Time Ontology."@en ;
                  rdfs:comment "Cardinality [0..1]. The value of this property is the (estimated) time needed for executing a Public Service which may depend on the Channel chosen . The actual information is provided using the ISO8601 syntax for durations."@en ,
                               "Cardinality [0..1]. The value of this property is the (estimated) time needed for executing a Public Service. The actual information is provided using the ISO8601 syntax for durations."@en ;
                  rdfs:label "processing time"@en .


###  http://data.europa.eu/m8g/telephone
cv:telephone rdf:type owl:DatatypeProperty ;
             rdfs:range rdf:langString ;
             rdfs:comment "Cardinality [0..n]. the telephone of the ContactPoint"@en ;
             rdfs:label "has telephone"@en .


###  http://purl.org/dc/terms/description
dct:description rdf:type owl:DatatypeProperty ;
                rdfs:range rdf:langString ;
                rdfs:comment "Cardinality [0..n]. This property represents a free text Description of the Output."@en ,
                             "Cardinality [0..n]. This property represents a free text Description of the piece of Evidence."@en ,
                             "Cardinality [0..n]. This property represents a free text description of the Cost."@en ,
                             "Cardinality [0..n]. This property represents a free text description of the Event. The description is likely to be the text that a business or citizen sees for that specific Event when looking for relevant Public Services. Public administrations are therefore encouraged to include a reasonable level of detail in the description."@en ,
                             "Cardinality [1..n]. A free text description of the Participation."@en ,
                             "Cardinality [1..n]. This property contains a free-text account of the Dataset. This property can be repeated for parallel language versions of the description."@en ,
                             "Cardinality [1..n]. This property represents a free text Description of the Public Service. The description is likely to be the text that potential users of the Public Service see in any public service catalogue. Public administrations are encouraged to include a reasonable level of detail in the description, for instance including basic eligibility requirements for the particular Public Service and contact information."@en ,
                             "Cardinality [1..n]. This property represents a free text Description of the Rule."@en ;
                rdfs:label "description"@en .


###  http://purl.org/dc/terms/title
dct:title rdf:type owl:DatatypeProperty ;
          rdfs:range rdf:langString ;
          rdfs:comment "Cardinality [1..n]. This property contains a name given to the Public Service Dataset. This property can be repeated for parallel language versions of the name."@en ,
                       "Cardinality [1..n]. This property represents the Name (or title) of the Event."@en ,
                       "Cardinality [1..n]. This property represents the Name of the Agent."@en ,
                       "Cardinality [1..n]. This property represents the Name of the Rule."@en ,
                       "Cardinality [1..n]. This property represents the official Name of the Output."@en ,
                       "Cardinality [1..n]. This property represents the official Name of the Public Service."@en ,
                       "Cardinality [1..n]. This property represents the official Name of the Requirement."@en ,
                       "Cardinality [1..n]. This property represents the official Name of the piece of Evidence."@en ;
          rdfs:label "name"@en .


###  http://www.w3.org/2004/02/skos/core#prefLabel
skos:prefLabel rdf:type owl:DatatypeProperty ;
               rdfs:range rdf:langString ;
               vann:usageNote "The value should be a URI from the Administrative Territorial Units Authority Table maintained by the Publications Office. (https://op.europa.eu/en/web/eu-vocabularies/dataset/-/resource?uri=http://publications.europa.eu/resource/dataset/atu)"@en ;
               rdfs:comment "Cardinality [1..1]. A Public Service is likely to be available only within a given area, typically the area covered by a particular public authority."@en ;
               rdfs:label "preferred label"@en .


###  http://www.w3.org/ns/dcat#keyword
dcat:keyword rdf:type owl:DatatypeProperty ;
             rdfs:range rdf:langString ;
             rdfs:comment "Cardinality [0..n]. This property represents a keyword, term or phrase to describe the Public Service."@en ;
             rdfs:label "keyword"@en .


###  http://www.w3.org/ns/locn#addressArea
locn:addressArea rdf:type owl:DatatypeProperty ;
                 rdfs:range rdf:langString ;
                 vann:usageNote "This would typically be part of a city, a neighbourhood or village, e.g. Montmartre."@en ;
                 rdfs:comment "Cardinality [0..n]. The name or names of a geographic area or locality that groups a number of addressable objects for addressing purposes, without being an administrative unit."@en ;
                 rdfs:label "address area"@en .


###  http://www.w3.org/ns/locn#addressID
locn:addressID rdf:type owl:DatatypeProperty ;
               rdfs:range xsd:string ;
               vann:usageNote """The concept of adding a globally unique identifier for each instance of an address is a crucial part of the INSPIRE data spec. A number of EU countries have already implemented an ID (a UUID) in their Address Register/gazetteer, among them Denmark. OASIS xAL also includes an address identifier. It is the address Identifier that allows an address to be represented in a format other than INSPIRE whilst remaining conformant to the Core Vocabulary.


The INSPIRE method of representing addresses is very detailed, designed primarily for use in databases of addresses. Whilst data that is published in full conformance with the INSPIRE data structure can be made available using the Location Core Vocabulary the reverse is not true since the Core Vocabulary allows much greater flexibility.


Many datasets that include address data as one piece of information about something else are likely to have that data in simpler formats. These might be tailored to the specific need of the dataset, follow a national norm, or make use of a standard like vCard.


To provide maximum flexibility in the Core Vocabulary, whilst remaining interoperable with INSPIRE Address Guidelines (which EU Member States are obliged to use), the Location Core Vocabulary provides the extra property of full address and makes use of INSPIRE's addressID."""@en ;
               rdfs:comment "Cardinality [0..n]. A globally unique identifier for each instance of an Address."@en ;
               rdfs:label "address ID"@en .


###  http://www.w3.org/ns/locn#adminUnitL1
locn:adminUnitL1 rdf:type owl:DatatypeProperty ;
                 rdfs:range rdf:langString ;
                 vann:usageNote """Best practice is to use the ISO 3166-1 code but if this is inappropriate for the context, country names should be provided in a consistent manner to reduce ambiguity. For example, either write 'France' or 'FRA' consistently throughout the dataset and avoid mixing the two. The Country controlled vocabulary from the Publications Office can be reused for this.
https://op.europa.eu/en/web/eu-vocabularies/dataset/-/resource?uri=http://publications.europa.eu/resource/dataset/country"""@en ;
                 rdfs:comment "Cardinality [0..n]. The name of the uppermost level of the address, almost always a country."@en ;
                 rdfs:label "administrative unit level 1 (country)"@en .


###  http://www.w3.org/ns/locn#adminUnitL2
locn:adminUnitL2 rdf:type owl:DatatypeProperty ;
                 rdfs:range rdf:langString ;
                 vann:usageNote "Values could be a region or province, more granular than level 1."@en ;
                 rdfs:comment "Cardinality [0..n]. The name of a secondary level/region of the address, usually a county, state or other such area that typically encompasses several localities."@en ;
                 rdfs:label "administrative unit level 2 (country/region/state)"@en .


###  http://www.w3.org/ns/locn#fullAddress
locn:fullAddress rdf:type owl:DatatypeProperty ;
                 rdfs:range rdf:langString ;
                 vann:usageNote "Use of this property is recommended as it will not suffer any misunderstandings that might arise through the breaking up of an address into its component parts. This property is analogous to vCard's label property but with two important differences: (1) formatting is not assumed so that, unlike vCard label, it may not be suitable to print this on an address label, (2) vCard's label property has a domain of vCard Address; the fullAddress property has no such restriction. An example of a full address is \"Champ de Mars, 5 Avenue Anatole France, 75007 Paris, France\"."@en ;
                 rdfs:comment "Cardinality [0..n]. The complete address written as a formatted string."@en ;
                 rdfs:label "full address"@en .


###  http://www.w3.org/ns/locn#locatorDesignator
locn:locatorDesignator rdf:type owl:DatatypeProperty ;
                       rdfs:range xsd:string ;
                       vann:usageNote "In simpler terms, this is the building number, apartment number, etc. For an address such as \"Flat 3, 17 Bridge Street\", the locator is \"flat 3, 17\"."@en ;
                       rdfs:comment "Cardinality [0..n]. A number or a sequence of characters which allows a user or an application to interpret, parse and format the locator within the relevant scope. A locator may include more locator designators"@en ;
                       rdfs:label "locator designator"@en .


###  http://www.w3.org/ns/locn#locatorName
locn:locatorName rdf:type owl:DatatypeProperty ;
                 rdfs:range rdf:langString ;
                 vann:usageNote """The locator name could be the name of the property or complex, of the building or part of the building, or it could be the name of a room inside a building.

The key difference between a locator and a locator name is that the latter is a proper name and is unlikely to include digits. For example, \"Schuman, Berlaymont\" is a meeting room within the European Commission headquarters for which locator name is more appropriate than locator."""@en ;
                 rdfs:comment "Cardinality [0..n]. Proper noun(s) applied to the real world entity identified by the locator."@en ;
                 rdfs:label "locator name"@en .


###  http://www.w3.org/ns/locn#poBox
locn:poBox rdf:type owl:DatatypeProperty ;
           rdfs:range xsd:string ;
           vann:usageNote "INSPIRE's name for this is \"postalDeliveryIdentifier\" for which it uses the locator designator property with a type attribute of that name. This vocabulary separates out the Post Office Box for greater independence of technology. An example post office box number is \"9383\"."@en ;
           rdfs:comment "Cardinality [0..n]. The Post Office Box number."@en ;
           rdfs:label "post office box"@en .


###  http://www.w3.org/ns/locn#postCode
locn:postCode rdf:type owl:DatatypeProperty ;
              rdfs:range xsd:string ;
              vann:usageNote "Post codes are common elements in many countries' postal address systems. One of the many post codes of Paris is for example \"75000\"."@en ;
              rdfs:comment "Cardinality [0..n]. The post/zip code of an address. (INSPIRE's definition is \"A code created and maintained for postal purposes to identify a subdivision of addresses and postal delivery points.\")"@en ;
              rdfs:label "post code"@en .


###  http://www.w3.org/ns/locn#postName
locn:postName rdf:type owl:DatatypeProperty ;
              rdfs:range rdf:langString ;
              rdfs:comment "Cardinality [0..n]. The key postal division of the address, usually the city. (INSPIRE's definition is \"One or more names created and maintained for postal purposes to identify a subdivision of addresses and postal delivery points.) For example, \"Paris\"."@en ;
              rdfs:label "post name (city)"@en .


###  http://www.w3.org/ns/locn#thoroughfare
locn:thoroughfare rdf:type owl:DatatypeProperty ;
                  rdfs:range rdf:langString ;
                  vann:usageNote "For example, \"Avenue des Champs-Élysées\"."@en ;
                  rdfs:comment "Cardinality [0..n]. An address component that represents the name or names of a passage or way through from one location to another. A thoroughfare is not necessarily a road, it might be a waterway or some other feature."@en ;
                  rdfs:label "thoroughfare"@en .


###  http://purl.org/dc/terms/identifier
<http://purl.org/dc/terms/identifier> rdf:type owl:DatatypeProperty ;
                                       rdfs:range rdf:langString .


###  http://purl.org/dc/terms/title
<http://purl.org/dc/terms/title> rdf:type owl:DatatypeProperty ;
                                  rdfs:range rdf:langString ;
                                  vann:usageNote "This property can be repeated for parallel language versions of the name."@en ;
                                  rdfs:comment "Cardinality [1..n]. This property contains a name given to the Dataset."@en ;
                                  rdfs:label "title"@en .


#################################################################
#    Classes
#################################################################

###  http://data.europa.eu/eli/ontology#LegalResource
eli:LegalResource rdf:type owl:Class ;
                  vann:usageNote "The definition and properties of the Legal Resource class in the CPSV-AP are aligned with the ontology included in \"Council conclusions inviting the introduction of the European Legislation Identifier (ELI)\". For describing the attributes of a Legal Resource (labels, preferred labels, alternative labels, definition ...) we refer to the ELI ontology."@en ;
                  rdfs:comment "Optional class. This class represents the legislation, policy or policies that lie behind the Rules that govern the service."@en ;
                  rdfs:isDefinedBy eli: ;
                  rdfs:label "Legal Resource"@en .


###  http://data.europa.eu/m8g/BusinessEvent
cv:BusinessEvent rdf:type owl:Class ;
                 rdfs:subClassOf cv:Event ;
                 rdfs:comment "Optional class. This class represents a Business Event, which specialises Event. A Business Event is a specific situation or event in the lifecycle of a business that fulfils one or more needs or (legal) obligations of that business at this specific point in time. A Business Event requires a set of public services to be delivered and consumed in order for the associated business need(s) or obligation(s) to be fulfilled. Business Events are defined within the context of a particular Member State. In other words, a Business Event groups together a number of public services that need to be delivered for completing that particular event."@en ;
                 rdfs:isDefinedBy <http://data.europa.eu/m8g/cpsvap> ;
                 rdfs:label "Business Event"@en .


###  http://data.europa.eu/m8g/Channel
cv:Channel rdf:type owl:Class ;
           rdfs:comment "Optional class. The Channel class represents the medium through which an Agent provides, uses or interacts in another way with a Public Service. Typical examples include online services, phone, walk-in centres etc."@en ;
           rdfs:isDefinedBy cv: ;
           rdfs:label "Channel"@en .


###  http://data.europa.eu/m8g/ContactPoint
cv:ContactPoint rdf:type owl:Class ;
                vann:usageNote "Similarly to the Channel class, a Contact Point may have regular opening hours that are then overridden by, for example, public holidays, using the Opening Hours Specification class."@en ;
                rdfs:comment "Optional class. This class represents the contact information for a Public Service, Channel, Public Organization, etc."@en ;
                rdfs:isDefinedBy cv: ;
                rdfs:label "Contact Point"@en .


###  http://data.europa.eu/m8g/Cost
cv:Cost rdf:type owl:Class ;
        rdfs:comment "Optional class. The Cost class represents any costs related to the execution of a Public Service that the Agent consuming it needs to pay."@en ;
        rdfs:isDefinedBy <http://data.europa.eu/m8g/cpsvap> ;
        rdfs:label "Cost"@en .


###  http://data.europa.eu/m8g/Event
cv:Event rdf:type owl:Class ;
         rdfs:comment "Optional class. This class represents an event that can be of any type that triggers, makes use of, or in some way is related to, a Public Service.  It is not expected to be used directly, rather, one or other of its subclasses should be used. The properties of the class are, of course, inherited by those subclasses."@en ;
         rdfs:isDefinedBy <http://data.europa.eu/m8g/cpsvap> ;
         rdfs:label "Event"@en .


###  http://data.europa.eu/m8g/Evidence
cv:Evidence rdf:type owl:Class ;
            vann:usageNote "Although the wording of the definition is different, the semantics are an exact match for CPSV's Input class which it replaces. Evidence can be any resource - document, artefact - anything needed for executing the Public Service. In the context of Public Services, Evidence is usually administrative documents or completed application forms. A specific Public Service may require the presence of certain Evidence or combinations of Evidence in order to be delivered. In some cases, the Output of one service will be Evidence for another service. Such relationships should be described in the associated Rule(s)."@en ;
            rdfs:comment "Optional class. The Evidence class is defined in the Core Criterion and Core Evidence vocabulary (CCCEV) as any resource that can document or support a criterion response. It contains information that proves that a criterion requirement exists or is true, in particular evidences are used to prove that a specific criterion is met."@en ;
            rdfs:isDefinedBy cv: ;
            rdfs:label "Evidence"@en .


###  http://data.europa.eu/m8g/LifeEvent
cv:LifeEvent rdf:type owl:Class ;
             rdfs:subClassOf cv:Event ;
             rdfs:comment "Optional class. The Life Event class represents an important event or situations in a citizen's life where public services may be required. Note the scope: an individual will encounter any number of 'events' in the general sense of the word. In the context of the CPSV-AP, the Life Event class only represents an event for which a Public Service is related. For example, a couple becoming engaged is not a CPSV-AP Life Event, getting married is, since only the latter has any relevance to public services."@en ;
             rdfs:isDefinedBy <http://data.europa.eu/m8g/cpsvap> ;
             rdfs:label "Life Event"@en .


###  http://data.europa.eu/m8g/OpeningHoursSpecification
cv:OpeningHoursSpecification rdf:type owl:Class ;
                             vann:usageNote "This class is aligned to Schema.org OpeningHoursSpecification class The Opening Hours Specification class can be used to provide details of exceptional circumstances, such as being closed on public holidays, which is encoded (in Turtle), thus: ex:PublicHolidayClosed a schema:OpeningHoursSpecification; schema:dayOfWeek . Note that the property schema:opens is not used, therefore the contact point is closed. More specific closures can be indicated by including the schema:validFrom and schema:validThrough properties, for example: ex:ChristmasClosed a schema:OpeningHoursSpecification; schema:validFrom \"2016-12-24T012:00Z\"; schema:validThrough \"2017-01-02T09:00Z\"."@en ;
                             rdfs:comment "Optional class. An exceptional circumstance that overrides the normal Opening Hours, such as being closed on public holidays."@en ;
                             rdfs:isDefinedBy <https://schema.org/> ;
                             rdfs:label "Opening Hours Specification"@en .


###  http://data.europa.eu/m8g/Output
cv:Output rdf:type owl:Class ;
          vann:usageNote "In some cases, the Output of one Public Service will be used as evidence to fulfil a criterion requirement of another Public Service. Such relationships should be described in the associated Rule(s)."@en ;
          rdfs:comment "Optional class. Outputs can be any resource - document, artefact – anything produced by the Public Service. In the context of a Public Service, the output provides an official document or other artefact of the Competent Authority (Public Organisation) that permits/authorises/entitles an Agent to (do) something."@en ;
          rdfs:isDefinedBy cpsv: ;
          rdfs:label "Output"@en .


###  http://data.europa.eu/m8g/Participation
cv:Participation rdf:type owl:Class ;
                 rdfs:comment "Optional class. The CPSV-AP recognises a common role connected with public services, i.e. the Competent Authority. However, this simple structure does not allow statements to be made about those participants, such the start and end date of a contract, nor does it support the inclusion of other roles. The Participation class supports this extra complexity if required, for instance, the description of a service user or a service provider. The model is consistent with the CPOV which in turn is based on the W3C Organization Ontology that supports the common cases simply but allows the complex cases where necessary. The Participation class can be mapped to the Organization Ontology's Membership class that allows more complex relationships and richer metadata to be applied to a role filled by a given Agent."@en ;
                 rdfs:isDefinedBy cv: ;
                 rdfs:label "Participation"@en .


###  http://data.europa.eu/m8g/PublicOrganisation
cv:PublicOrganisation rdf:type owl:Class ;
                      rdfs:subClassOf org:Organization ;
                      vann:usageNote "Organizations which exist to provide services for its citizens and companies are called Public Organizations. The Public Organization class represents the organization. One organization may comprise several sub-organizations and any organization may have one or more organizational units. Each of these is described using the same properties and relationships. This definition is consistent with the more detailed definition of a \"public sector body\" as given in the PSI Directive: \"the State, regional or local authorities, bodies governed by public law and associations formed by one or several such authorities or one or several such bodies governed by public law\". It further defines a body governed by public law as any body \"(a) established for the specific purpose of meeting needs in the general interest, not having an industrial or commercial character; and (b) having legal personality; and (c) financed, for the most part by the State, or regional or local authorities, or other bodies governed by public law; or subject to management supervision by those bodies; or having an administrative, managerial or supervisory board, more than half of whose members are appointed by the State, regional or local authorities or by other bodies governed by public law\"."@en ;
                      rdfs:comment "Mandatory class. Any Organization that is defined as being part of the public sector by a legal framework at any level."@en ;
                      rdfs:isDefinedBy cv: ;
                      rdfs:label "Public Organisation"@en .


###  http://data.europa.eu/m8g/Requirement
cv:Requirement rdf:type owl:Class ;
               vann:usageNote """Not all public services are needed or usable by everyone. For example, the visa service operated by European countries is not needed by European citizens but is needed by some citizens from elsewhere, or public services offering unemployment benefits and grants are targeting specific societal groups. The CPSV-AP reuses the Core Criterion and Core Evidence Vocabulary for this class.

Requirement is a generic class representing any type of prerequisite that may be desired, needed or imposed as an obligation. CCCEV recommends to not use the Requirement class directly, but rather a more semantically-enriched subclass such as Criterion, Information Requirement or Constraint. Also note that the Requirement class is specified at a more abstract level and is not to be used as the instantiation of a Requirement for a specific Agent.
To illustrate the notion: the European Directive on services in the internal market defines requirement as any obligation, prohibition, condition or limit provided for in the laws, regulations or administrative provisions of the Member States or in consequence of case-law, administrative practice, the rules of professional bodies, or the collective rules of professional associations or other professional organisations, adopted in the exercise of their legal autonomy."""@en ;
               rdfs:comment "Optional class. Condition or prerequisite that is to be proven by Evidence."@en ;
               rdfs:isDefinedBy cv: ;
               rdfs:label "Requirement"@en .


###  http://purl.org/vocab/cpsv#PublicService
cpsv:PublicService rdf:type owl:Class ;
                   rdfs:comment "Mandatory class. This class represents the Public Service itself, as it is described in a public service catalogue. A Public Service is a mandatory or discretionary set of activities performed, or able to be performed, by or on behalf of a public organisation, publicly funded and arise from public policy. Services may be for the benefit of an individual, a business, or other public authority, or groups of any of these. A service exists whether it is used or not, and the term 'benefit' may apply in the sense of enabling the fulfilment of an obligation. As defined in the revised version of the European Interoperability Framework, a European public service comprises any service provided by public administrations in Europe, or by other organisations on their behalf, to businesses, citizens or others public administrations."@en ;
                   rdfs:isDefinedBy cpsv: ;
                   rdfs:label "Public Service"@en .


###  http://purl.org/vocab/cpsv#Rule
cpsv:Rule rdf:type owl:Class ;
          rdfs:comment "Optional class. The Rule class represents a document that sets out the specific rules, guidelines or procedures that the Public Service follows. It includes the terms of service, licence, and authentication requirements of the Public Service. Instances of the Rule class are FRBR Expressions, that is, a concrete expression such as a document, of the more abstract concept of the rules themselves. The CPSV-AP does not envisage instances of the Rule class as machine-readable business rules. Detailed modelling of the rules related to Public Services is out of scope of the CPSV-AP."@en ;
          rdfs:isDefinedBy cpsv: ;
          rdfs:label "Rule"@en .


###  http://www.w3.org/2004/02/skos/core#Collection
skos:Collection rdf:type owl:Class ;
                rdfs:comment "Optional class. This class represents the Collection to which a Concept belongs. Grouping different concepts defines a controlled vocabulary. In this context the CPSV-AP reuses the Collection  class as defined in the SKOS Simple Knowledge Organization System . For describing the attributes of a Collection (labels, preferred labels, alternative labels, definition …) we refer to SKOS."@en ;
                rdfs:isDefinedBy skos: ;
                rdfs:label "Collection"@en .


###  http://www.w3.org/2004/02/skos/core#Concept
skos:Concept rdf:type owl:Class ;
             rdfs:comment "Optional class. This class represents any concept that can be used for classifying the Public Service and which relates to the Public Service through the property Is Classified By. This class has been added in the CPSV-AP to complement the need for adding other ways of classifying the Public Service, which have not been explicitely defined in the CPSV-AP. In this context the CPSV-AP reuses the Concept  class as defined in the SKOS Simple Knowledge Organization System . For describing the attributes of a Concept (labels, preferred labels, alternative labels, definition …) we refer to SKOS. The Concept may or may not belong to (member) a certain Collection."@en ;
             rdfs:isDefinedBy skos: ;
             rdfs:label "Concept"@en .


###  http://www.w3.org/ns/locn#Address
locn:Address rdf:type owl:Class ;
             vann:usageNote """An \"address representation\" as conceptually defined by the INSPIRE Address Representation data type: \"Representation of an address spatial object for use in external application schemas that need to include the basic, address information in a readable way.\"


The representation of Addresses varies widely from one country's postal system to another. Even within countries, there are almost always examples of Addresses that do not conform to the stated national standard. At the time of publication, work is progressing on ISO 19160-1 that defines a method through which different Addresses can be converted from one conceptual model to another.


This specification was heavily based on the INSPIRE Address Representation data type. It is noteworthy that if an Address is provided using the detailed breakdown suggested by the properties for this class, then it will be INSPIRE-conformant. To this very granular set of properties, we add two further properties:

- full address (the complete address as a formatted string)
- addressID (a unique identifier for the address)
The first of these allows publishers to simply provide the complete Address as one string, with or without formatting. This is analogous to vCard's label property.

The addressID is part of the INSPIRE guidelines and provides a hook that can be used to link the Address to an alternative representation, such as vCard or OASIS xAL."""@en ;
             rdfs:comment "Optional class. A spatial object that identifies a fixed location of a property, in a human-readable way."@en ;
             rdfs:isDefinedBy locn: ;
             rdfs:label "Address"@en .


###  http://www.w3.org/ns/org#Organization
org:Organization rdf:type owl:Class ;
                 rdfs:comment "Represents a collection of people organized together into a community or other social, commercial or political structure. The group has some common purpose or reason for existence which goes beyond the set of people belonging to it and can act as an Agent. Organizations are often decomposable into hierarchical structures.  It is recommended that SKOS lexical labels should be used to label the Organization. In particular `skos:prefLabel` for the primary (possibly legally recognized name), `skos:altLabel` for alternative names (trading names, colloquial names) and `skos:notation` to denote a code from a code list. Alternative names: _Collective_ _Body_ _Org_ _Group_"@en ;
                 rdfs:label "Organization"@en .


###  http://xmlns.com/foaf/0.1/Agent
foaf:Agent rdf:type owl:Class ;
           rdfs:comment "Optional class. The Agent class is any resource that acts or has the power to act. This includes people, organisations and groups. The Public Organization class, defined in the Core Public Organisation Vocabulary, is a notable subclass of Agent."@en ;
           rdfs:isDefinedBy foaf: ;
           rdfs:label "Agent"@en .


###  http://purl.org/dc/terms/LinguisticSystem
<http://purl.org/dc/terms/LinguisticSystem> rdf:type owl:Class ;
                                             rdfs:comment "Optional class. A system of signs, symbols, sounds, gestures, or rules used in communication."@en ;
                                             rdfs:isDefinedBy dct: ;
                                             rdfs:label "Linguistic System"@en .


###  http://purl.org/dc/terms/Location
<http://purl.org/dc/terms/Location> rdf:type owl:Class ;
                                     rdfs:comment "Optional class. An identifiable geographic place or named place."@en ;
                                     rdfs:isDefinedBy dct: ;
                                     rdfs:label "Location"@en .


###  https://www.w3.org/ns/dcat#Dataset
<https://www.w3.org/ns/dcat#Dataset> rdf:type owl:Class ;
                                     rdfs:comment "Optional class. The class describes the metada of where the dataset is being described, for instance on a regional public service portal and/or a national eGovernment portal."@en ;
                                     rdfs:isDefinedBy <https://www.w3.org/ns/dcat#> ;
                                     rdfs:label "Dataset"@en .


###  http://xmlns.com/foaf/0.1/Document
<http://xmlns.com/foaf/0.1/Document> rdf:type owl:Class ;
                                      rdfs:comment "Optional class. A document."@en ;
                                      rdfs:isDefinedBy foaf: ;
                                      rdfs:label "Document"@en .


#################################################################
#    Individuals
#################################################################

###  http://data.europa.eu/m8g/cpsvap
<http://data.europa.eu/m8g/cpsvap> rdf:type owl:NamedIndividual ;
                                   dct:publisher <http://publications.europa.eu/resource/authority/corporate-body/DIGIT> ;
                                   adms:status <http://purl.org/adms/status/Completed> ;
                                   dct:description "The original CPSV-AP was prepared in the context of Action 1.3 – Accessing Member State information resources at European level – Catalogue of Services  of the European Commission’s Interoperability for European Public Administrations (ISA) programme. The CPSV-AP has been seen as a first step for creating a model for describing public services related to business events, to facilitate the set-up of catalogues of services in the context of the Services Directive. Update to version 2.2 finds its motivation in the experience of implementing version 2.1 of the CPSV-AP by different MSs and stakeholders and consequent requests received from them, as detailed in https://github.com/catalogue-of-services-isa/CPSV-AP/issues."@en ;
                                   dct:title "Core Public Service Vocabulary Application Profile"@en .


###  http://publications.europa.eu/resource/authority/corporate-body/DIGIT
<http://publications.europa.eu/resource/authority/corporate-body/DIGIT> rdf:type owl:NamedIndividual .


###  http://purl.org/adms/assettype/Ontology
<http://purl.org/adms/assettype/Ontology> rdf:type owl:NamedIndividual .


###  http://purl.org/adms/status/Completed
<http://purl.org/adms/status/Completed> rdf:type owl:NamedIndividual .


###  http://purl.org/dc/terms/identifier
<http://purl.org/dc/terms/identifier> rdf:type owl:NamedIndividual ;
                                       dct:description "Recommended best practice is to identify the resource by means of a string conforming to a formal identification system. "@en .


#################################################################
#    Annotations
#################################################################

<http://purl.org/dc/terms/identifier> rdfs:comment "An unambiguous reference to the resource within a given context."@en ,
                                                    "Cardinality [1..1]. This property represents a formally-issued Identifier for the Public Service."@en ,
                                                    "Cardinality [1..1]. This property represents an Identifier for the Rule."@en ;
                                       dct:hasVersion <http://dublincore.org/usage/terms/history/#identifierT-001> ;
                                       rdfs:comment "Cardinality [1..1]. This property represents an Identifier for the Event."@en ,
                                                    "Cardinality [1..1]. This property represents an Identifier for the Cost."@en ;
                                       rdfs:isDefinedBy dct: ;
                                       rdfs:comment "Cardinality [1..1]. This property represents an Identifier for the piece of Evidence."@en ,
                                                    "Cardinality [1..1]. This property represents an Identifier for the Participation."@en ,
                                                    "Cardinality [1..1]. This property represents an Identifier for the Output."@en ,
                                                    "Cardinality [1..1]. This property represents an Identifier for the Agent."@en ,
                                                    "Cardinality [0..n]. This property contains the main identifier for the Dataset, e.g. the URI or other unique identifier in the context of the Catalogue."@en ,
                                                    "Cardinality [1..1]. This property represents an Identifier for the Channel."@en ,
                                                    "Cardinality [1..1]. This property represents an Identifier for the Requirement."@en ;
                                       rdfs:label "identifier"@en .


#################################################################
#    General axioms
#################################################################

[ rdf:type owl:AllDifferent ;
  owl:distinctMembers ( <http://data.europa.eu/m8g/cpsvap>
                        <http://publications.europa.eu/resource/authority/corporate-body/DIGIT>
                        <http://purl.org/adms/assettype/Ontology>
                        <http://purl.org/dc/terms/identifier>
                      )
] .


###  Generated by the OWL API (version 4.5.9.2019-02-01T07:24:44Z) https://github.com/owlcs/owlapi
